# baseURI: http://tno.io/Classifications
# imports: http://www.ontology-of-units-of-measure.org/resource/om-2/
# imports: http://www.w3.org/2004/02/skos/core
# imports: http://www.w3.org/ns/shacl#
# prefix: classifications

@prefix : <http://tno.io/Classifications#> .
@prefix DT: <http://tno.io/DigitalTwin#> .
@prefix MathM: <http://www.w3.org/1998/Math/MathML> .
@prefix businessService: <http://tno.io/BusinessService#> .
@prefix classifications: <http://tno.io/Classifications#> .
@prefix om: <http://www.ontology-of-units-of-measure.org/resource/om-2/#> .
@prefix owl: <http://www.w3.org/2002/07/owl#> .
@prefix rdf: <http://www.w3.org/1999/02/22-rdf-syntax-ns#> .
@prefix rdfs: <http://www.w3.org/2000/01/rdf-schema#> .
@prefix sh: <http://www.w3.org/ns/shacl#> .
@prefix skos: <http://www.w3.org/2004/02/skos/core#> .
@prefix xsd: <http://www.w3.org/2001/XMLSchema#> .

<http://tno.io/Classifications>
  rdf:type owl:Ontology ;
  owl:imports <http://www.ontology-of-units-of-measure.org/resource/om-2/> ;
  owl:imports <http://www.w3.org/2004/02/skos/core> ;
  owl:imports sh: ;
.
classifications:Air
  rdf:type classifications:transportModality ;
.
classifications:Atlantic_Corridor
  rdf:type classifications:corridorName ;
.
classifications:Baltic-Adriatic_Corridor
  rdf:type classifications:corridorName ;
.
classifications:D
  rdf:type classifications:natureOfCargo ;
  rdfs:label "Dangerous" ;
.
classifications:D_1
  rdfs:label "Reefer" ;
.
classifications:E
  rdf:type classifications:natureOfCargo ;
  rdfs:label "Excise" ;
.
classifications:Explosives
  rdf:type classifications:dangerouseGoodCode ;
  rdf:type skos:Concept ;
  rdf:type skos:ConceptScheme ;
.
classifications:FCL-FCL
  rdf:type classifications:transportMovementType ;
  rdfs:comment """FCL/FCL
Defines the movement of cargo packed by the shipper or shipper's agent and unpacked by the consignee or consignee's agent. 'FCL' means Full Container Load.""" ;
.
classifications:Flammable_Gases
  rdf:type classifications:dangerouseGoodCode ;
  rdf:type skos:Concept ;
  rdf:type skos:ConceptScheme ;
.
classifications:H200
  rdf:type classifications:dangerouseGoodCode ;
  rdf:type skos:Concept ;
  rdfs:comment "based on https://www.unece.org/fileadmin/DAM/trans/danger/publi/ghs/ghs_rev07/English/05e_annex1.pdf" ;
  skos:topConceptOf classifications:Explosives ;
.
classifications:H201
  rdf:type classifications:dangerouseGoodCode ;
  rdf:type skos:Concept ;
  skos:broader classifications:Explosives ;
.
classifications:H220
  rdf:type classifications:dangerouseGoodCode ;
  rdf:type skos:Concept ;
  skos:topConceptOf classifications:Flammable_Gases ;
.
classifications:LCL-LCL
  rdf:type classifications:transportMovementType ;
  rdfs:comment "Defines the movement of cargo packed in and unpacked from containers by the carrier on behalf of the shipper/consignee. 'LCL' means Less than Container Load." ;
.
classifications:Mediterranean_Corridor
  rdf:type classifications:corridorName ;
.
classifications:North_Sea-Baltic_Corridor
  rdf:type classifications:corridorName ;
.
classifications:North_Sea-Mediterranean_Corridor
  rdf:type classifications:corridorName ;
.
classifications:Orient_East-Med_Corridor
  rdf:type classifications:corridorName ;
.
classifications:Palletized
  rdf:type classifications:packageType ;
.
classifications:R
  rdf:type classifications:natureOfCargo ;
  rdfs:label "Reefer" ;
.
classifications:Rhine-Alpine_Corridor
  rdf:type classifications:corridorName ;
.
classifications:Rhine-Danube_Corridor
  rdf:type classifications:corridorName ;
.
classifications:Rhine_Alpine_Corridor
  rdf:type classifications:corridorName ;
.
classifications:Road
  rdf:type classifications:transportModality ;
.
classifications:Scandinavian-Mediterranean_Corridor
  rdf:type classifications:corridorName ;
.
classifications:Sea
  rdf:type classifications:transportModality ;
.
classifications:W
  rdf:type classifications:natureOfCargo ;
  rdfs:label "Waste" ;
.
classifications:appliesTo
  rdf:type owl:ObjectProperty ;
.
classifications:cargoType
  rdf:type owl:Class ;
  rdfs:comment "classifies types of cargo. For instance large freight container." ;
  rdfs:subClassOf classifications:classifications ;
.
classifications:classifications
  rdf:type owl:Class ;
  rdfs:subClassOf owl:Thing ;
.
classifications:corridorName
  rdf:type owl:Class ;
  rdfs:comment """Core network corridors\" were introduced to facilitate the coordinated implementation of the core network in Europe. 

Nine core network corridors are identified in the annex to the CEF Regulation, which includes a list of projects pre-identified for possible EU funding during the period 2014 â€“ 2020, based on their added value for TEN-T development and their maturity status.""" ;
  rdfs:subClassOf classifications:classifications ;
.
classifications:dangerouseGoodCode
  rdf:type owl:Class ;
  rdfs:comment """Danger and Hazard classification, labeling and codification based on UN classifications -- https://www.unece.org/fileadmin/DAM/trans/danger/publi/ghs/ghs_rev07/English/05e_annex1.pdf
For the scope of proof of concept we selected only few example just to demonstrate the capability of the model.""" ;
  rdfs:subClassOf classifications:classifications ;
.
classifications:dangerouseGoodsClassification
  rdf:type owl:ObjectProperty ;
.
classifications:large_freight_container
  rdf:type classifications:cargoType ;
.
classifications:natureOfCargo
  rdf:type owl:Class ;
  rdfs:comment "This class classifies the codes or vocbualries that express the nature of cargo." ;
  rdfs:subClassOf classifications:classifications ;
.
classifications:packageType
  rdf:type owl:Class ;
  rdfs:comment "It classifies the vocbularies for expressing types of packages." ;
  rdfs:subClassOf classifications:classifications ;
.
classifications:transportModality
  rdf:type owl:Class ;
  rdfs:comment """The various modes used for a movement. For each mode, there are several means of transport. They are: a. inland surface transportation (rail, road, and inland waterway); b. sea transport (coastal and ocean); c. air transportation; and d. pipelines. 
For the purpose of the usecase, we encode the top individulas only. Sea, Road, Air.""" ;
  rdfs:subClassOf classifications:classifications ;
.
classifications:transportMovementType
  rdf:type owl:Class ;
  rdfs:comment "This is to specify transport movement details for a goods item or equipment. For the purpose of this project ,we selected only few examples to demonstrate in the proof of concept -- the complete list can be found here:https://www.stylusstudio.com/edifact/D04B/8335.htm" ;
  rdfs:subClassOf classifications:classifications ;
.
