# baseURI: http://tno.io/DigitalTwin

@prefix : <http://tno.io/DigitalTwin#> .
@prefix DT: <http://tno.io/DigitalTwin#> .
@prefix event: <http://tno.io/Event#> .
@prefix businessService: <http://tno.io/BusinessService#> .
@prefix owl: <http://www.w3.org/2002/07/owl#> .
@prefix rdf: <http://www.w3.org/1999/02/22-rdf-syntax-ns#> .
@prefix rdfs: <http://www.w3.org/2000/01/rdf-schema#> .
@prefix xsd: <http://www.w3.org/2001/XMLSchema#> .

DT:
  rdf:type owl:Ontology ;
  owl:imports businessService: ;
  owl:imports event: ;
  owl:imports <http://www.w3.org/2004/02/skos/core> ;
  owl:versionInfo "Created with TopBraid Composer"^^xsd:string ;
 .
 
DT:DigitalTwin
  rdf:type owl:Class ;
  rdfs:subClassOf owl:Thing ;
  .

DT:Actor  a                owl:Class ;
	rdfs:comment     "The role of a Person is context dependant, and therefore should be described using the Actor class." ;
	rdfs:subClassOf  DT:DigitalTwin ;
	.

DT:Cargo  a                owl:Class ;
       rdfs:comment     "The goods that are transported from origin to destination." ;
       rdfs:subClassOf  DT:DigitalTwin ;
       .

DT:Equipment  a            owl:Class ;
        rdfs:comment     "Any asset used to facilitate transport and handling of cargo." ;
        rdfs:subClassOf  DT:DigitalTwin ;
        .
DT:Location  a             owl:Class ;
        rdfs:comment     "A terminal, location, port, city centre, etc. where a cargo physical activity like transhipment or storage can take place." ;
        rdfs:subClassOf  DT:DigitalTwin ;
        .
DT:Product  a              owl:Class ;
        rdfs:comment     "The actual objects that change ownership between a seller to a buyer. Any commercial goods that is bought and sold."^^xsd:string ;
        rdfs:subClassOf  DT:DigitalTwin ;
        .
DT:Role   a                rdfs:Class ;
		rdfs:comment     "" ;
        rdfs:subClassOf  DT:DigitalTwin ;
        .
DT:Transportmeans  a       owl:Class ;
        rdfs:comment     "These are the vehicles that transport the cargo, such as tricks, vessels,\r\ntrains, airplanes, barges etc." ;
        rdfs:subClassOf  DT:DigitalTwin ;
        .
 
DT:Organization  a         owl:Class ;
        rdfs:subClassOf  DT:Actor ;
        .
        
 
DT:Authority  a            owl:Class ;
        rdfs:subClassOf  DT:Organization ;
        .


DT:CertificationAuthority
        a                owl:Class ;
        rdfs:subClassOf  DT:Organization ;
        .


DT:Enterprise  a           owl:Class ;
        rdfs:subClassOf  DT:Organization ;
        .
        
DT:Person  a               owl:Class ;
        rdfs:comment     "Any individual that is a crew on board of a transport means." , "The role of a Person should not be defined here, but in its linked Actor class." ;
        rdfs:subClassOf  DT:Actor ;
        .
  
DT:bulkCargo  a            owl:Class ;
        rdfs:subClassOf  DT:Cargo ;
        .
        

DT:containerizedCargo  a   owl:Class ;
        rdfs:subClassOf  DT:Cargo ;
        .
DT:generalCargo  a         owl:Class ;
        rdfs:subClassOf  DT:Cargo ;
        .
      
DT:Container  a            owl:Class ;
        rdfs:comment     "Transport containers serve to containerize products." ;
        rdfs:subClassOf  DT:Equipment ;
        .
        
DT:RailwayWagon  a         owl:Class ;
        rdfs:comment     "Unpowered railway vehicles that are used for the transportation of cargo." ;
        rdfs:subClassOf  DT:Equipment ;
        .

DT:Swapbody  a             owl:Class ;
        rdfs:subClassOf  DT:Equipment ;
        .
        
DT:Trailer  a              owl:Class ;
        rdfs:comment     "Unpowered road vehicles that are used for the transportation of cargo." ;
        rdfs:subClassOf  DT:Equipment ;
        .
 
 
DT:ULD    a                owl:Class ;
        rdfs:comment     "Unit Load Devices are light weight containers for air transport and facilitate loading cargo into aircraft." ;
        rdfs:subClassOf  DT:Equipment .
 


:InfrastructuralFunction
        a                 owl:Class ;
        rdfs:comment      "Any part of an infrastructure used for performing logistical activities." ;
        rdfs:subClassOf   :Location ;
        owl:disjointWith  :LogisticalFunction ;
        .
        
 :Area   a                owl:Class ;
        rdfs:comment     "Any area relevant to logistics operations." ;
        rdfs:subClassOf  :InfrastructuralFunction ;
        .
        
 :InfrastructuralObject
        a                owl:Class ;
        rdfs:subClassOf  :InfrastructuralFunction ;
        .
 
 
:City   a                owl:Class ;
        rdfs:comment     "A generic geographical location." ;
        rdfs:subClassOf  :InfrastructuralFunction ;
        .
 


:other_InfrastructuralLocation  a                owl:Class ;
        rdfs:subClassOf  :InfrastructuralFunction ;
         .
      
:Trajectory  a           owl:Class ;
        rdfs:comment     "Any part of an infrastructure identified by its infrastructure manager." ;
        rdfs:subClassOf  :InfrastructuralFunction ;
        .
 
 :landmark  a             owl:Class ;
        rdfs:subClassOf  :Location ;
        .
 

:LogisticalFunction  a   owl:Class ;
        rdfs:comment     "Any location where a logistical activity is performed." ;
        rdfs:subClassOf  :Location ;
        .


:Airport  a              owl:Class ;
        rdfs:comment     "Location where airplanes pick or drop of freight." ;
        rdfs:subClassOf  :LogisticalFunction ;
        .


:anchorage  a            owl:Class ;
        rdfs:subClassOf  :LogisticalFunction ;
        .


:Hub    a                owl:Class ;
        rdfs:comment     "A place cargo is exchanged between vehicles or/and between transport modes." ;
        rdfs:subClassOf  :LogisticalFunction ;
        .
        
  
:Terminal  a             owl:Class ;
        rdfs:comment     "A freight terminal for different modes is a processing node for freight." ;
        rdfs:subClassOf  :Hub ;
        .
        
 
:Port   a                owl:Class ;
        rdfs:comment     "Location where vessels pick or drop of freight." ;
        rdfs:subClassOf  :LogisticalFunction ;
        .
        
:Transshipment  a        owl:Class ;
        rdfs:comment     "An intermediate destination for transiting cargo to another destination." ;
        rdfs:subClassOf  :LogisticalFunction ;
        .
        

:bulkProduct  a          owl:Class ;
        rdfs:comment     "Any unpackaged raw material"^^xsd:string ;
        rdfs:subClassOf  :Product ;
        .
        
  
:commercialProduct  a    owl:Class ;
        rdfs:comment     "Any product destined for use by enterprise. Consumer products may be packaged in quantities."^^xsd:string ;
        rdfs:subClassOf  :Product ;
        .
        
DT:consumerProduct  a      owl:Class ;
        rdfs:comment     "Any product destined for consumption or use by consumers. Consumer products might be packaged in quantities."^^xsd:string ;
        rdfs:subClassOf  DT:Product ;
        .
        
 DT:partProduct  a          owl:Class ;
        rdfs:comment     "Products destined for use in machines owned by consumers or enterprises"^^xsd:string ;
        rdfs:subClassOf  :Product ;
        .
        
  DT:business_roles  a       rdfs:Class ;
        rdfs:subClassOf  :Role ;
        .
        
DT:infrastructural_roles
        a                rdfs:Class ;
        rdfs:subClassOf  :Role ;
        .
 
  DT:location_role  a        owl:Class ;
        rdfs:subClassOf  DT:Role ;
        .
        
 :orgnizational_roles  a  rdfs:Class ;
        rdfs:subClassOf  :Role .
 
  
:Transportation_role  a  rdfs:Class ;
        rdfs:subClassOf  :Role ;
        .
        
 :Airplane  a             owl:Class ;
        rdfs:comment     "Transport means by air." ;
        rdfs:subClassOf  :Transportmeans ;
        .
        
 :Barge  a                owl:Class ;
        rdfs:comment     "Vessel used for transporting cargo on inland waterways." ;
        rdfs:subClassOf  :Transportmeans ;
        .
  
  :Locomotive  a           owl:Class ;
        rdfs:comment     "Any traction for a train composed of one or more wagons." ;
        rdfs:subClassOf  :Transportmeans ;
        .

:Truck  a                owl:Class ;
        rdfs:comment     "Any transport means for road transport." ;
        rdfs:subClassOf  :Transportmeans ;
        .
  
  
:Vessel  a               owl:Class ;
        rdfs:comment     "Any transport means used for transporting cargo by sea/ocean." ;
        rdfs:subClassOf  :Transportmeans ;
        .
        
 :DeepseaVessel  a        owl:Class ;
        rdfs:comment     "Used for ocean transport." ;
        rdfs:subClassOf  :Vessel ;
        .
        
 :DeepseaBulkVessel  a    owl:Class ;
        rdfs:subClassOf  :DeepseaVessel ;
       .
       
 :DeepseaContainerVessel
        a                owl:Class ;
        rdfs:subClassOf  :DeepseaVessel ;
        .
        
        
  :Feeder  a               owl:Class ;
        rdfs:comment     "Used for short range transport  via sea." ;
        rdfs:subClassOf  :Vessel ;
        .
        
 :BulkFeeder  a           owl:Class ;
        rdfs:subClassOf  :Feeder ;
        .
        
:ContainerFeeder  a      owl:Class ;
        rdfs:subClassOf  :Feeder ;
        .
        
:Ferry  a                owl:Class ;
        rdfs:comment     "Used for transport of other transport means like trucks and/or trailers." ;
        rdfs:subClassOf  :Vessel ;
        .
:Ferry  a                owl:Class ;
        rdfs:comment     "Used for transport of other transport means like trucks and/or trailers." ;
        rdfs:subClassOf  :Vessel ;
        .        
        
        
   ################################################
   ####3DataType PROPERTIES####
   ##############################################   
        
:bulk_volume  a      owl:DatatypeProperty ;
        rdfs:domain  :bulkCargo ;
        rdfs:range   xsd:integer .
 
:cargo_container_number
        a            owl:DatatypeProperty ;
        rdfs:domain  :containerizedCargo ;
        rdfs:range   xsd:string .
 
:cargo_container_size
        a            owl:DatatypeProperty ;
        rdfs:domain  :containerizedCargo ;
        rdfs:range   xsd:integer .
        
        
:cargo_container_type
        a            owl:DatatypeProperty ;
        rdfs:domain  :containerizedCargo ;
        rdfs:range   xsd:string .
 
:damage_location  a  owl:DatatypeProperty ;
        rdfs:domain  :containerizedCargo ;
        rdfs:range   xsd:string .
 
:damage_remarks  a   owl:DatatypeProperty ;
        rdfs:domain  :containerizedCargo ;
        rdfs:range   xsd:string .
        
        
:equipment_container_ITU_code
        a            owl:DatatypeProperty ;
        rdfs:domain  :Container ;
        rdfs:range   xsd:string .
        
:equipment_container_size
        a            owl:DatatypeProperty ;
        rdfs:domain  :Container ;
        rdfs:range   xsd:string .
 
:equipment_container_tare_weight
        a            owl:DatatypeProperty ;
        rdfs:domain  :Container ;
        rdfs:range   xsd:integer .
        
:equipment_container_type
        a            owl:DatatypeProperty ;
        rdfs:domain  :Container ;
        rdfs:range   xsd:string .
 

:euqipment_trailer_license_plate
        a            owl:DatatypeProperty ;
        rdfs:domain  :Trailer ;
        rdfs:range   xsd:string .

 
 :goods_description  a  owl:DatatypeProperty ;
        rdfs:domain  :generalCargo ;
        rdfs:range   xsd:string .
 
 
 :grossMass  a        owl:DatatypeProperty ;
        rdfs:domain  :generalCargo ;
        rdfs:range   xsd:integer .
 
 
 :is_empty  a         owl:DatatypeProperty ;
        rdfs:domain  :RailwayWagon , :containerizedCargo ;
        rdfs:range   xsd:boolean .
 
 :is_full  a     owl:DatatypeProperty ;
        rdfs:domain  :RailwayWagon ;
        rdfs:range   xsd:boolean .
 
 
:locomotive_brake_type  a     owl:DatatypeProperty ;
        rdfs:domain  :Locomotive ;
        rdfs:range   xsd:string .
        
        
:locomotive_brake_weight   a     owl:DatatypeProperty ;
        rdfs:domain  :Locomotive ;
        rdfs:range   xsd:string .

 
 
:locomotive_driver_indication   a    owl:DatatypeProperty ;
        rdfs:domain  :Locomotive ;
        rdfs:range   xsd:string .
 
 
 
:locomotive_identifier     a     owl:DatatypeProperty ;
        rdfs:domain  :Locomotive ;
        rdfs:range   xsd:string .
 
 
 
:locomotive_traction_type   a    owl:DatatypeProperty ;
        rdfs:domain  :Locomotive ;
        rdfs:range   xsd:string .
 
 
:locomotive_type_number    a     owl:DatatypeProperty ;
        rdfs:domain  :Locomotive ;
        rdfs:range   xsd:string .
  
  
:marks_number  a     owl:DatatypeProperty ;
        rdfs:domain  :generalCargo ;
        rdfs:range   xsd:string .
  
  
:measure  a          owl:DatatypeProperty ;
        rdfs:domain  :generalCargo ;
        rdfs:range   xsd:integer .
    
    
:modality  a         owl:DatatypeProperty ;
        rdfs:domain  :Transportmeans ;
        rdfs:range   xsd:string .
  
  
:netLoad  a          owl:DatatypeProperty ;
        rdfs:domain  :containerizedCargo ;
        rdfs:range   xsd:integer .
    
  
:netMass  a          owl:DatatypeProperty ;
        rdfs:domain  :generalCargo ;
        rdfs:range   xsd:integer .
    
        
:numberofPackages  a  owl:DatatypeProperty ;
        rdfs:domain  :generalCargo ;
        rdfs:range   xsd:integer .
      


:package_level_type  a  owl:DatatypeProperty ;
        rdfs:domain  :generalCargo ;
        rdfs:range   xsd:string .
        
        
:package_type  a     owl:DatatypeProperty ;
        rdfs:domain  :generalCargo ;
        rdfs:range   xsd:string .
 
 
:product_ID  a        owl:DatatypeProperty ;
        rdfs:comment  "Code uniquely identifying a product from either customer or service provider (supplier) perspective."^^xsd:string ;
        rdfs:range    xsd:string .
        
        
:product_Name  a      owl:DatatypeProperty ;
        rdfs:comment  "Name of the product related to the code"^^xsd:string ;
        rdfs:range    xsd:string .
        
:security_level  a   owl:DatatypeProperty ;
        rdfs:domain  :Port ;
        rdfs:range   xsd:string .
        
        
:security_measure  a  owl:DatatypeProperty ;
        rdfs:domain  :Port ;
        rdfs:range   xsd:string .
        
        
:shipping_marks  a   owl:DatatypeProperty ;
        rdfs:domain  :generalCargo ;
        rdfs:range   xsd:string .
        
  
:CargoSize   a            owl:DatatypeProperty ;
        rdfs:domain  :Cargo ;
        rdfs:range   xsd:integer .
        
:truck_license_plate  a  owl:DatatypeProperty ;
        rdfs:domain  :Truck ;
        rdfs:range   xsd:string .
        
 
:vessel_name  a      owl:DatatypeProperty ;
        rdfs:domain  :Vessel ;
        rdfs:range   xsd:string .
        
:vessel_type  a      owl:DatatypeProperty ;
        rdfs:domain  :Vessel ;
        rdfs:range   xsd:string .
        
 
:wagon_brake_type  a  owl:DatatypeProperty ;
        rdfs:domain  :RailwayWagon ;
        rdfs:range   xsd:string .
        
        
:wagon_brake_weight  a  owl:DatatypeProperty ;
        rdfs:domain  :RailwayWagon ;
        rdfs:range   xsd:integer .
        
        
:wagon_maximum_speed  a  owl:DatatypeProperty ;
        rdfs:domain  :RailwayWagon ;
        rdfs:range   xsd:integer .
        
:wagon_nr_axel  a    owl:DatatypeProperty ;
        rdfs:domain  :RailwayWagon ;
        rdfs:range   xsd:string .
        
        
        
        
        
        
        
        
        
        
        
        