# baseURI: https://ontology.tno.nl/logistics/federated/BusinessService
# imports: https://ontology.tno.nl/logistics/federated/LogisticsRoles
# prefix: businessService

@prefix : <https://ontology.tno.nl/logistics/federated/BusinessService#> .
@prefix Classifications: <https://ontology.tno.nl/logistics/federated/Classifications#> .
@prefix DigitalTwin: <https://ontology.tno.nl/logistics/federated/DigitalTwin#> .
@prefix Event: <https://ontology.tno.nl/logistics/federated/Event#> .
@prefix LogisticsRoles: <https://ontology.tno.nl/logistics/federated/LogisticsRoles#> .
@prefix ReusableTags: <https://ontology.tno.nl/logistics/federated/ReusableTags#> .
@prefix businessService: <https://ontology.tno.nl/logistics/federated/BusinessService#> .
@prefix dc: <http://purl.org/dc/elements/1.1/> .
@prefix dcterms: <http://purl.org/dc/terms/> .
@prefix owl: <http://www.w3.org/2002/07/owl#> .
@prefix pi: <https://ontology.tno.nl/logistics/federated/PhysicalInfrastructure#> .
@prefix rdf: <http://www.w3.org/1999/02/22-rdf-syntax-ns#> .
@prefix rdfs: <http://www.w3.org/2000/01/rdf-schema#> .
@prefix skos: <http://www.w3.org/2004/02/skos/core#> .
@prefix xsd: <http://www.w3.org/2001/XMLSchema#> .

<https://ontology.tno.nl/logistics/federated/BusinessService>
  a owl:Ontology ;
  dc:creator "Dena Tahvildari, Maaike Burghoorn, Cornelis Bouter" ;
  dcterms:created "2020-07-20" ;
  dcterms:description "This ontology contains classes, attributes, relation about business services that are used in Logistics events." ;
  dcterms:isRequiredBy <https://ontology.tno.nl/logistics/federated/Event> ;
  dcterms:issued "2021-03-15" ;
  dcterms:language "en" ;
  dcterms:requires <https://ontology.tno.nl/logistics/federated/Classifications> ;
  dcterms:requires <https://ontology.tno.nl/logistics/federated/LogisticsRoles> ;
  #owl:imports <https://ontology.tno.nl/logistics/federated/LogisticsRoles> ;
  #owl:versionIRI <https://ontology.tno.nl/logistics/federated/BusinessServicev-0.1> ;
  owl:versionInfo "Created with TopBraid Composer" ;
.
businessService:Booking
  a owl:Class ;
  rdfs:comment "Agreement with a limited validity period between two enterprises for one or more orders" ;
  rdfs:label "Booking" ;
  rdfs:subClassOf businessService:BusinessTransaction ;
.
businessService:BusinessTransaction
  a owl:Class ;
  rdfs:comment "All data shared by interactions for executing a business service" ;
  rdfs:label "Business Transaction" ;
  rdfs:subClassOf owl:Thing ;
.
businessService:Consignment
  a owl:Class ;
  rdfs:comment "A consignment is a business transaction of a shipper as customer with a service provider (e.g. a carrier or forwarder) for the transport of goods or containers from one location to another, where all goods and containers have to arrive in a given time period. The time period indicates that the goods or containers can arrive with different transport means at different times, but they all have to present after the period has ended." ;
  rdfs:label "Consignment" ;
  rdfs:subClassOf businessService:BusinessTransaction ;
  rdfs:subClassOf [
      a owl:Restriction ;
      owl:minQualifiedCardinality "1"^^xsd:nonNegativeInteger ;
      owl:onClass businessService:LegalPerson ;
      owl:onProperty businessService:involvedActor ;
    ] ;
  rdfs:subClassOf [
      a owl:Restriction ;
      owl:minQualifiedCardinality "1"^^xsd:nonNegativeInteger ;
      owl:onClass Classifications:GoodsTypeCode ;
      owl:onProperty DigitalTwin:goodsTypeCode ;
    ] ;
  rdfs:subClassOf [
      a owl:Restriction ;
      owl:minQualifiedCardinality "1"^^xsd:nonNegativeInteger ;
      owl:onClass Classifications:TransportMovementType ;
      owl:onProperty businessService:partOfTransportMovementType ;
    ] ;
  rdfs:subClassOf [
      a owl:Restriction ;
      owl:minQualifiedCardinality "1"^^xsd:nonNegativeInteger ;
      owl:onClass DigitalTwin:Goods ;
      owl:onProperty businessService:usedGoods ;
    ] ;
  rdfs:subClassOf [
      a owl:Restriction ;
      owl:minQualifiedCardinality "1"^^xsd:nonNegativeInteger ;
      owl:onClass DigitalTwin:Package ;
      owl:onProperty businessService:usedPackage ;
    ] ;
  rdfs:subClassOf [
      a owl:Restriction ;
      owl:minQualifiedCardinality "1"^^xsd:nonNegativeInteger ;
      owl:onClass DigitalTwin:Equipment ;
      owl:onProperty businessService:usedTransportEquipment ;
    ] ;
  rdfs:subClassOf [
      a owl:Restriction ;
      owl:minQualifiedCardinality "1"^^xsd:nonNegativeInteger ;
      owl:onDataRange xsd:integer ;
      owl:onProperty DigitalTwin:numberofPackages ;
    ] ;
  rdfs:subClassOf [
      a owl:Restriction ;
      owl:minQualifiedCardinality "1"^^xsd:nonNegativeInteger ;
      owl:onDataRange xsd:string ;
      owl:onProperty businessService:hasSequenceNumber ;
    ] ;
  ReusableTags:isDerived true ;
.
businessService:Enterprise
  a owl:Class ;
  rdfs:comment "A business or a company" ;
  rdfs:label "Enterprise" ;
  rdfs:subClassOf businessService:LegalEntity ;
.
businessService:FrameworkContract
  a owl:Class ;
  rdfs:comment "A contract with a long term validity period between any two enterprise with agreements of business service delivery" ;
  rdfs:label "Framework Contract" ;
  rdfs:subClassOf businessService:BusinessTransaction ;
.
businessService:Itinerary
  a owl:Class ;
  rdfs:comment "A timed sequence of places of call of a transport means. Potentially, an itinerary has a unique ID, e.g. voyage number and flight number." ;
  rdfs:label "Itinerary" ;
  rdfs:subClassOf owl:Thing ;
  rdfs:subClassOf [
      a owl:Restriction ;
      owl:minQualifiedCardinality "1"^^xsd:nonNegativeInteger ;
      owl:onClass DigitalTwin:TransportMeans ;
      owl:onProperty businessService:involves ;
    ] ;
  rdfs:subClassOf [
      a owl:Restriction ;
      owl:minQualifiedCardinality "1"^^xsd:nonNegativeInteger ;
      owl:onClass Event:Event ;
      owl:onProperty businessService:involves ;
    ] ;
  rdfs:subClassOf [
      a owl:Restriction ;
      owl:minQualifiedCardinality "1"^^xsd:nonNegativeInteger ;
      owl:onClass pi:LogisticalFunction ;
      owl:onProperty businessService:involves ;
    ] ;
  rdfs:subClassOf [
      a owl:Restriction ;
      owl:minQualifiedCardinality "1"^^xsd:nonNegativeInteger ;
      owl:onDataRange xsd:string ;
      owl:onProperty businessService:itineraryID ;
    ] ;
  ReusableTags:isDerived true ;
.
businessService:LegalEntity
  a owl:Class ;
  rdfs:label "Legal entity" ;
  rdfs:comment "An entity processing separate and distinct legal rights." ;
  rdfs:subClassOf businessService:LegalPerson ;
  skos:prefLabel "Legal entity" ;
.
businessService:LegalPerson
  a owl:Class ;
  rdfs:subClassOf owl:Thing ;
  rdfs:comment "The role of a Person, Enterprise or Organization is context dependant, and therefore should be described using the LogisticsRoles:Roles class." ;
  rdfs:label "Logistics Actor" ;
  rdfs:subClassOf [
      a owl:Restriction ;
      owl:minQualifiedCardinality "1"^^xsd:nonNegativeInteger ;
      owl:onDataRange xsd:string ;
      owl:onProperty businessService:actorName ;
    ] ;
  rdfs:subClassOf [
      a owl:Restriction ;
      owl:minQualifiedCardinality "1"^^xsd:nonNegativeInteger ;
      owl:onDataRange xsd:string ;
      owl:onProperty businessService:actorWebsite ;
    ] ;
  rdfs:subClassOf [
      a owl:Restriction ;
      owl:minQualifiedCardinality "1"^^xsd:nonNegativeInteger ;
      owl:onClass pi:Location ;
      owl:onProperty businessService:actorAddress ;
    ] ;
.
businessService:LogisticsService
  a owl:Class ;
  rdfs:comment "Any service that is provided to a customer by a logistics or transport service provider." ;
  rdfs:label "Logistics Service" ;
  rdfs:subClassOf owl:Thing ;
.
businessService:LogisticsServiceGroupage
  a owl:Class ;
  rdfs:comment "A service for grouping of cargo into equipment" ;
  rdfs:label "Groupage Service" ;
  rdfs:subClassOf businessService:LogisticsService ;
.
businessService:NaturalPerson
  a owl:Class ;
  rdfs:comment "An individual human being" ;
  rdfs:label "Person" ;
  rdfs:subClassOf businessService:LegalPerson ;
.
businessService:Order
  a owl:Class ;
  rdfs:comment "Agreement between two enterprise for actual execution of a business service according a booking or framework contract." ;
  rdfs:label "Order" ;
  rdfs:subClassOf businessService:BusinessTransaction ;
.
businessService:Organization
  a owl:Class ;
  rdfs:comment "An agent corresponding to social institutions such as companies, societies etc." ;
  rdfs:label "Organization" ;
  rdfs:subClassOf businessService:LegalEntity ;
.
businessService:PrivateEnterprise
  a owl:Class ;
  rdfs:comment "A private business or company" ;
  rdfs:label "Private Enterprise" ;
  rdfs:subClassOf businessService:Enterprise ;
.
businessService:PublicEnterprise
  a owl:Class ;
  rdfs:comment "A public business or company" ;
  rdfs:label "Public Enterprise" ;
  rdfs:subClassOf businessService:Enterprise ;
.
businessService:Route
  a owl:Class ;
  rdfs:comment "The use of infrastructure (sea, road, rail etc.) taken by transport means between any two locations of its itinerary." ;
  rdfs:label "Route" ;
  rdfs:subClassOf owl:Thing ;
  rdfs:subClassOf [
      a owl:Restriction ;
      owl:minQualifiedCardinality "1"^^xsd:nonNegativeInteger ;
      owl:onClass DigitalTwin:TransportMeans ;
      owl:onProperty businessService:involves ;
    ] ;
  rdfs:subClassOf [
      a owl:Restriction ;
      owl:minQualifiedCardinality "1"^^xsd:nonNegativeInteger ;
      owl:onClass Event:Event ;
      owl:onProperty businessService:involves ;
    ] ;
  rdfs:subClassOf [
      a owl:Restriction ;
      owl:minQualifiedCardinality "1"^^xsd:nonNegativeInteger ;
      owl:onClass pi:InfrastructuralFunction ;
      owl:onProperty businessService:involves ;
    ] ;
  ReusableTags:isDerived true ;
.
businessService:Shipment
  a owl:Class ;
  rdfs:comment "A shipment is a business transaction with a carrier for the transport of goods or containers from one location to another, where all goods and containers have to arrive in a given time period. This is similar to a consignment; however, it is always a carrier acting as service provider." ;
  rdfs:label "Shipment" ;
  rdfs:subClassOf owl:Thing ;
  ReusableTags:isDerived true ;
.
businessService:StorageServiceCargo
  a owl:Class ;
  rdfs:comment "A service for (temporary) storage of cargo. This may include special cargo storage such as cool storage, animal hotels, and dangerous goods storage." ;
  rdfs:label "Storage Service Cargo" ;
  rdfs:subClassOf businessService:LogisticsService ;
.
businessService:StorageServiceProduct
  a owl:Class ;
  rdfs:comment "A service for storage of products (warehousing)" ;
  rdfs:label "Storage Service Product" ;
  rdfs:subClassOf businessService:LogisticsService ;
.
businessService:TransportService
  a owl:Class ;
  rdfs:comment "A service provided by a logistics for transport of cargo" ;
  rdfs:label "Transport Service" ;
  rdfs:subClassOf businessService:LogisticsService ;
.
businessService:TransshipmentService
  a owl:Class ;
  rdfs:comment "A service for transshipping cargo from one transport means to another" ;
  rdfs:label "Transshipment Service" ;
  rdfs:subClassOf businessService:LogisticsService ;
.
businessService:actorID
  a owl:DatatypeProperty ;
  rdfs:comment "ID of the logistics actor" ;
  rdfs:domain businessService:LegalPerson ;
  rdfs:label "Actor ID" ;
  rdfs:range xsd:string ;
.
businessService:actorName
  a owl:DatatypeProperty ;
  rdfs:comment "Name of the logistics actor" ;
  rdfs:domain businessService:LegalPerson ;
  rdfs:label "Actor name" ;
  rdfs:range xsd:string ;
.
businessService:actorWebsite
  a owl:DatatypeProperty ;
  rdfs:comment "URL of the website of the logistics actor" ;
  rdfs:domain businessService:LegalPerson ;
  rdfs:label "Actor website" ;
  rdfs:range xsd:string ;
.
businessService:bookingNumber
  a owl:DatatypeProperty ;
  rdfs:comment "Booking number of the booking business transaction" ;
  rdfs:domain businessService:Booking ;
  rdfs:label "Booking number" ;
  rdfs:range xsd:string ;
.
businessService:HasBookingStatus
  a owl:ObjectProperty ;
  rdfs:comment "The relationship between booking and booking status" ;
  rdfs:domain businessService:Booking ;
  rdfs:label "Booking Status" ;
  rdfs:range businessService:BookingStatus;
.
businessService:consignmentCreationTime
  a owl:DatatypeProperty ;
  rdfs:comment "Time that Consigment is created" ;
  rdfs:domain businessService:Consignment ;
  rdfs:label "consignment Creation Time" ;
  rdfs:range xsd:dateTime ;
.
businessService:consignmentUpdateTime
  a owl:DatatypeProperty ;
  rdfs:comment "Time that Consigment is Updated" ;
  rdfs:domain businessService:Consignment ;
  rdfs:label "consignment Update Time" ;
  rdfs:range xsd:dateTime ;
.
businessService:createdBy
  a owl:DatatypeProperty ;
  rdfs:comment "Creator of business transaction and its types for example booking" ;
  rdfs:domain businessService:BusinessTransaction ;
  rdfs:label "Created By" ;
  rdfs:range xsd:string ;
.
businessService:deviationDuration
  a owl:DatatypeProperty ;
  rdfs:comment "Deviation on the duration of the transport service" ;
  rdfs:domain businessService:TransportService ;
  rdfs:label "Deviation duration" ;
  rdfs:range xsd:decimal ;
.
businessService:hasLocation
  rdfs:comment "Location of the logistics service" ;
  rdfs:label "has location" ;
  rdfs:domain businessService:LogisticsService ;
  rdfs:range pi:Location ;
.
businessService:hasSequenceNumber
  a owl:DatatypeProperty ;
  rdfs:domain businessService:BusinessTransaction ;
  rdfs:label "Has Sequence Number" ;
  rdfs:comment "The relationship between the business transaction and its sequence number expressed as a string" ;
  rdfs:range xsd:string ;
.
businessService:hasService
  a owl:ObjectProperty ;
  rdfs:comment "Business transaction is part of a logistics service" ;
  rdfs:domain businessService:BusinessTransaction ;
  rdfs:label "Has service" ;
  rdfs:range businessService:LogisticsService ;
.
businessService:actorAddress
  a owl:ObjectProperty ;
  rdfs:comment "Address of the logistics actor" ;
  rdfs:domain businessService:LegalPerson ;
  rdfs:label "Actor address" ;
  rdfs:range pi:Location ;
.
businessService:involvedActor
  a owl:ObjectProperty ;
  rdfs:comment "An Enterprise, Person or Organization can have different roles depending on the context. This property and its subproperties define the different roles that legal persons can play in the context of a business transaction." ;
  rdfs:domain businessService:BusinessTransaction ;
  rdfs:label "Involved actor" ;
  rdfs:range businessService:LegalPerson ;
  rdfs:subPropertyOf businessService:involves ;
.
businessService:involvedAuthority
  a owl:ObjectProperty ;
  rdfs:label "involved authority" ;
  rdfs:comment "The realtionship between a business transaction and an authority that has been instantiated as a businessService:legalperson."; 
  rdfs:subPropertyOf businessService:involvedCommercialActor ;
.
businessService:involvedBank
  a owl:ObjectProperty ;
  rdfs:label "involved bank" ;
  rdfs:comment "The realtionship between a business transaction and a bank that has been instantiated as a businessService:legalperson."; 
  rdfs:subPropertyOf businessService:involvedFinancialActor ;
.
businessService:involvedBusinessActor
  a owl:ObjectProperty ;
  rdfs:label "involved business person" ;
  rdfs:comment "The realtionship between a business transaction and a business actor that has been instantiated as a businessService:legalperson.";  
  rdfs:subPropertyOf businessService:involvedActor ;
.
businessService:involvedCarrier
  a owl:ObjectProperty ;
  rdfs:label "involved carrier" ;
  rdfs:comment "The realtionship between a business transaction and a carrier that has been instantiated as a businessService:legalperson."; 
  rdfs:subPropertyOf businessService:involvedLogisticsActor ;
.
businessService:involvedCommercialActor
  a owl:ObjectProperty ;
  rdfs:label "involved commercial person" ;
  rdfs:comment "The realtionship between a business transaction and a commercial actor that has been instantiated as a businessService:legalperson."; 
  rdfs:subPropertyOf businessService:involvedActor ;
.
businessService:involvedConsignee
  a owl:ObjectProperty ;
  rdfs:label "involved Consignee" ;
  rdfs:comment "The realtionship between a business transaction and a consignee that has been instantiated as a businessService:legalperson."; 
  rdfs:subPropertyOf businessService:involvedLogisticsActor ;
.
businessService:involvedConsignor
  a owl:ObjectProperty ;
  rdfs:label "involved Consignor" ;
  rdfs:comment "The realtionship between a business transaction and a consignor that has been instantiated as a businessService:legalperson."; 
  rdfs:subPropertyOf businessService:involvedLogisticsActor ;
.
businessService:involvedConsumer
  a owl:ObjectProperty ;
  rdfs:label "involved consumer" ;
  rdfs:comment "The realtionship between a business transaction and a consumer that has been instantiated as a businessService:legalperson."; 
  rdfs:subPropertyOf businessService:involvedSupplyChainActor ;
.
businessService:involvedContactPerson
  a owl:ObjectProperty ;
  rdfs:label "involved contact person" ;
  rdfs:comment "The realtionship between a business transaction and an involved contact person that has been instantiated as a businessService:legalperson."; 
  rdfs:subPropertyOf businessService:involvedCommercialActor ;
.
businessService:involvedCustomer
  a owl:ObjectProperty ;
  rdfs:label "involved customer" ;
  rdfs:comment "The realtionship between a business transaction and a customer that has been instantiated as a businessService:legalperson."; 
  rdfs:subPropertyOf businessService:involvedCommercialActor ;
.
businessService:involvedCustomsAuthority
  a owl:ObjectProperty ;
  rdfs:label "involved customs authority" ;
  rdfs:comment "The realtionship between a business transaction and an involved customs authority that has been instantiated as a businessService:legalperson."; 
  rdfs:subPropertyOf businessService:involvedAuthority ;
.
businessService:involvedDeclarant
  a owl:ObjectProperty ;
  rdfs:label "involved declarant" ;
  rdfs:comment "The realtionship between a business transaction and a declarant that has been instantiated as a businessService:legalperson."; 
  rdfs:subPropertyOf businessService:involvedBusinessActor ;
.
businessService:involvedDeliveryParty
  a owl:ObjectProperty ;
  rdfs:label "involved delivery party" ;
  rdfs:comment "The realtionship between a business transaction and an involved delivery party that has been instantiated as a businessService:legalperson."; 
  rdfs:subPropertyOf businessService:involvedLogisticsActor ;
.
businessService:involvedDispatchParty
  a owl:ObjectProperty ;
  rdfs:label "involved dispatch party" ;
  rdfs:comment "The realtionship between a business transaction and an involved dispatch party that has been instantiated as a businessService:legalperson."; 
  rdfs:subPropertyOf businessService:involvedLogisticsActor ;
.
businessService:involvedEvent
  a owl:ObjectProperty ;
  rdfs:comment "Event involved with business transaction" ;
  rdfs:domain businessService:BusinessTransaction ;
  rdfs:label "Involved event" ;
  rdfs:range Event:Event ;
  rdfs:subPropertyOf businessService:involves ;
.
businessService:involvedExporter
  a owl:ObjectProperty ;
  rdfs:label "involved exporter" ;
  rdfs:comment "The realtionship between a business transaction and an involved exporter that has been instantiated as a businessService:legalperson."; 
  rdfs:subPropertyOf businessService:involvedBusinessActor ;
.
businessService:involvedFinancialActor
  a owl:ObjectProperty ;
  rdfs:label "involved financial person" ;
  rdfs:comment "The realtionship between a business transaction and an involved financial actor that has been instantiated as a businessService:legalperson."; 
  rdfs:subPropertyOf businessService:involvedActor ;
.
businessService:involvedForwarder
  a owl:ObjectProperty ;
  rdfs:label "involved forwarder" ;
  rdfs:comment "The realtionship between a business transaction and an involved forwarder that has been instantiated as a businessService:legalperson."; 
  rdfs:subPropertyOf businessService:involvedLogisticsActor ;
.
businessService:involvedImporter
  a owl:ObjectProperty ;
  rdfs:label "involved importer" ;
  rdfs:comment "The realtionship between a business transaction and an involved importerer that has been instantiated as a businessService:legalperson."; 
  rdfs:subPropertyOf businessService:involvedBusinessActor ;
.
businessService:involvedInsurer
  a owl:ObjectProperty ;
  rdfs:label "involved insurer" ;
  rdfs:comment "The realtionship between a business transaction and an involved insurer that has been instantiated as a businessService:legalperson."; 
  rdfs:subPropertyOf businessService:involvedFinancialActor ;
.
businessService:involvedIssuer
  a owl:ObjectProperty ;
  rdfs:label "involved issuer" ;
  rdfs:comment "The realtionship between a business transaction and an involved issuer that has been instantiated as a businessService:legalperson."; 
  rdfs:subPropertyOf businessService:involvedBusinessActor ;
.
businessService:involvedLogisticsActor
  a owl:ObjectProperty ;
  rdfs:label "involved logistics actor" ;
  rdfs:comment "The realtionship between a business transaction and an involved logistics actor that has been instantiated as a businessService:legalperson."; 
  rdfs:subPropertyOf businessService:involvedActor ;
.
businessService:involvedLogisticsServiceProvider
  a owl:ObjectProperty ;
  rdfs:label "involved logistics service provider" ;
  rdfs:comment "The realtionship between a business transaction and an involved logistics service provider that has been instantiated as a businessService:legalperson."; 
  rdfs:subPropertyOf businessService:involvedLogisticsActor ;
.
businessService:involvedNotifyParty
  a owl:ObjectProperty ;
  rdfs:label "involved notify party" ;
  rdfs:comment "The realtionship between a business transaction and an involved notify party that has been instantiated as a businessService:legalperson."; 
  rdfs:subPropertyOf businessService:involvedLogisticsActor ;
.
businessService:involvedOperator
  a owl:ObjectProperty ;
  rdfs:label "involved operator" ;
  rdfs:comment "The realtionship between a business transaction and an involved operator that has been instantiated as a businessService:legalperson."; 
  rdfs:subPropertyOf businessService:involvedLogisticsActor ;
.
businessService:involvedPayee
  a owl:ObjectProperty ;
  rdfs:label "involved payee" ;
  rdfs:comment "The realtionship between a business transaction and an involved payee that has been instantiated as a businessService:legalperson."; 
  rdfs:subPropertyOf businessService:involvedFinancialActor ;
.
businessService:involvedPayer
  a owl:ObjectProperty ;
  rdfs:label "involved payer" ;
  rdfs:comment "The realtionship between a business transaction and an involved payer that has been instantiated as a businessService:legalperson."; 
  rdfs:subPropertyOf businessService:involvedFinancialActor ;
.
businessService:involvedPortAuthority
  a owl:ObjectProperty ;
  rdfs:label "involved port authority" ;
  rdfs:comment "The realtionship between a business transaction and an involved port authority that has been instantiated as a businessService:legalperson."; 
  rdfs:subPropertyOf businessService:involvedAuthority ;
.
businessService:involvedProducer
  a owl:ObjectProperty ;
  rdfs:label "involved producer" ;
  rdfs:comment "The realtionship between a business transaction and an involved producer that has been instantiated as a businessService:legalperson."; 
  rdfs:subPropertyOf businessService:involvedSupplyChainActor ;
.
businessService:involvedRetailer
  a owl:ObjectProperty ;
  rdfs:label "involved retailer" ;
  rdfs:comment "The realtionship between a business transaction and an involved retailer that has been instantiated as a businessService:legalperson."; 
  rdfs:subPropertyOf businessService:involvedSupplyChainActor ;
.
businessService:involvedSender
  a owl:ObjectProperty ;
  rdfs:label "involved sender" ;
  rdfs:comment "The realtionship between a business transaction and an involved sender that has been instantiated as a businessService:legalperson."; 
  rdfs:subPropertyOf businessService:involvedBusinessActor ;
.
businessService:involvedServiceProvider
  a owl:ObjectProperty ;
  rdfs:label "involved service provider" ;
  rdfs:comment "The realtionship between a business transaction and an involved service provider that has been instantiated as a businessService:legalperson."; 
  rdfs:subPropertyOf businessService:involvedCommercialActor ;
.
businessService:involvedShuntingYard
  a owl:ObjectProperty ;
  rdfs:label "involved shunting yard" ;
  rdfs:comment "The realtionship between a business transaction and an involved shunting yard that has been instantiated as a businessService:legalperson."; 
  rdfs:subPropertyOf businessService:involvedLogisticsActor ;
.
businessService:involvedSupplyChainActor
  a owl:ObjectProperty ;
  rdfs:label "involved supply chain actor" ;
  rdfs:comment "The realtionship between a business transaction and an involved supply chain actor that has been instantiated as a businessService:legalperson."; 
  rdfs:subPropertyOf businessService:involvedActor ;
.
businessService:involvedTerminalOperator
  a owl:ObjectProperty ;
  rdfs:label "involved terminal operator" ;
  rdfs:comment "The realtionship between a business transaction and an involved terminal operator that has been instantiated as a businessService:legalperson."; 
  rdfs:subPropertyOf businessService:involvedOperator ;
.
businessService:involvedWarehouseOperator
  a owl:ObjectProperty ;
  rdfs:label "involved warehouse operator" ;
  rdfs:comment "The realtionship between a business transaction and an involved warehouse operator that has been instantiated as a businessService:legalperson."; 
  rdfs:subPropertyOf businessService:involvedOperator ;
.
businessService:involves
  a owl:ObjectProperty ;
  rdfs:label "Involves" ;
  rdfs:comment "Abstract property -- do not instantiate" ;
.
businessService:itineraryID
  a owl:DatatypeProperty ;
  rdfs:comment "Each itinerary is assigned an unique ID" ;
  rdfs:domain businessService:Itinerary ;
  rdfs:label "Itinerary ID" ;
  rdfs:range xsd:string ;
  skos:altLabel "voyageID" ;
.
businessService:hasRole
  a owl:ObjectProperty ;
  rdfs:comment "The relationship between legal person and LogisticsRoles:ActorRoles" ;
  rdfs:domain businessService:LegalPerson ; 
  rdfs:label "has role" ;
  rdfs:range LogisticsRoles:ActorRoles ;
.

businessService:partOfTransportMovementType
  a owl:ObjectProperty ;
  rdfs:comment "Describes if the business transaction if part of main-, on-, or precarriage" ;
  rdfs:domain businessService:BusinessTransaction ;
  rdfs:label "Transport movement type" ;
  rdfs:range Classifications:TransportMovementType ;
.
businessService:serviceName
  a owl:DatatypeProperty ;
  rdfs:comment "Each type of logistics service can be described using a name." ;
  rdfs:domain businessService:LogisticsService ;
  rdfs:label "Service name" ;
  rdfs:range xsd:string ;
.
businessService:transportPlanIssuanceTime
  a owl:DatatypeProperty ;
  rdfs:comment "Date that the tranpsort service is issued." ;
  rdfs:domain businessService:BusinessTransaction ;
  rdfs:label "Transport Plan Issuance Time" ;
  rdfs:range xsd:dateTime ;
.
businessService:transportPlanSequenceNumber
  a owl:DatatypeProperty ;
  rdfs:comment "transport Plan Sequence Number" ;
  rdfs:domain businessService:BusinessTransaction ;
  rdfs:label "transport Plan Sequence Number" ;
  rdfs:range xsd:string ;
.
businessService:transportPlanTotalNumber
  a owl:DatatypeProperty ;
  rdfs:comment "transport Plan Total Number" ;
  rdfs:domain businessService:BusinessTransaction ;
  rdfs:label "transportPlanTotalNumber" ;
  rdfs:range xsd:string ;
.
businessService:transportServiceDurationAverage
  a owl:DatatypeProperty ;
  rdfs:comment "Each transport service has a average duration of completion" ;
  rdfs:domain businessService:TransportService ;
  rdfs:label "Transport service duration average" ;
  rdfs:range xsd:decimal ;
.
businessService:usedGoods
  a owl:ObjectProperty ;
  rdfs:comment "Goods that are part of the logistics service" ;
  rdfs:label "Used goods" ;
  rdfs:range DigitalTwin:Goods ;
.
businessService:usedPackage
  a owl:ObjectProperty ;
  rdfs:comment "Package that is part of the logistics service" ;
  rdfs:label "Used package" ;
  rdfs:range DigitalTwin:Package ;
.
businessService:usedPackagedProducts
  a owl:ObjectProperty ;
  rdfs:comment "Packaged products that are part of the logistics service" ;
  rdfs:domain businessService:LogisticsService ;
  rdfs:label "Package products" ;
.
businessService:usedTransportEquipment
  a owl:ObjectProperty ;
  rdfs:comment "Transport equipment involved with the logistics service" ;
  rdfs:label "Used transport equipment" ;
  rdfs:range DigitalTwin:Equipment ;
.
businessService:usedTransportMeans
  a owl:ObjectProperty ;
  rdfs:comment "Transports means involved with the logistics service" ;
  rdfs:domain businessService:LogisticsService ;
  rdfs:label "Used transport means" ;
  rdfs:range DigitalTwin:TransportMeans ;
.
businessService:usedTransportModality
  a owl:ObjectProperty ;
  rdfs:comment "Describes transport modality of the transport service" ;
  rdfs:domain businessService:TransportService ;
  rdfs:label "Used transport modality" ;
  rdfs:range Classifications:TransportModality ;
.

businessService:BookingStatus
  a owl:Class ;
  rdfs:comment "The booking status can be canceled, combined or active" ;
  rdfs:label "Booking Status" ;
.
businessService:canceled 
  a businessService:BookingStatus;
  rdfs:comment " Booking status: canceled";
  rdfs:label "canceled" ;
.
businessService:combined 
  a businessService:BookingStatus;
  rdfs:comment " Booking status: combined";
  rdfs:label "combined" ;
.
businessService:active 
  a businessService:BookingStatus;
  rdfs:comment " Booking status: active";
  rdfs:label "active" ;
.

DigitalTwin:goodsTypeCode a owl:ObjectProperty;
.

DigitalTwin:numberofPackages a owl:DatatypeProperty;
.
