# baseURI: https://ontology.tno.nl/logistics/federated/Classifications
# imports: http://www.w3.org/2004/02/skos/core
# imports: https://ontology.tno.nl/logistics/federated/DigitalTwin
# prefix: classifications

@prefix : <https://ontology.tno.nl/logistics/federated/Classifications#> .
@prefix DigitalTwin: <https://ontology.tno.nl/logistics/federated/DigitalTwin#> .
@prefix businessService: <https://ontology.tno.nl/logistics/federated/businessService#> .
@prefix classifications: <https://ontology.tno.nl/logistics/federated/Classifications#> .
@prefix dc: <http://purl.org/dc/elements/1.1/> .
@prefix dcterms: <http://purl.org/dc/terms/> .
@prefix owl: <http://www.w3.org/2002/07/owl#> .
@prefix rdf: <http://www.w3.org/1999/02/22-rdf-syntax-ns#> .
@prefix rdfs: <http://www.w3.org/2000/01/rdf-schema#> .
@prefix sh: <http://www.w3.org/ns/shacl#> .
@prefix skos: <http://www.w3.org/2004/02/skos/core#> .
@prefix xsd: <http://www.w3.org/2001/XMLSchema#> .

<https://ontology.tno.nl/logistics/federated/Classifications>
  rdf:type owl:Ontology ;
  dc:creator "Dena Tahvildari, Maaike Burghoorn, Cornelis Bouter" ;
  dcterms:created "2020-07-17" ;
  dcterms:description "This ontology contains classes, attributes, relation about from established standards and vocabularies relevant in the Logistics domain. It is intended to be reused by the other ontologies in the namespace." ;
  dcterms:isRequiredBy <https://ontology.tno.nl/logistics/federated/BusinessService> ;
  dcterms:isRequiredBy <https://ontology.tno.nl/logistics/federated/DigitalTwin> ;
  dcterms:isRequiredBy <https://ontology.tno.nl/logistics/federated/PhysicalInfrastructure> ;
  dcterms:issued "2021-03-15" ;
  dcterms:language "en" ;
  owl:imports <http://www.w3.org/2004/02/skos/core> ;
  owl:imports <https://ontology.tno.nl/logistics/federated/DigitalTwin> ;
  owl:versionIRI <https://ontology.tno.nl/logistics/federated/Classificationsv-0.1> ;
.
classifications:Air
  rdf:type classifications:TransportModality ;
.
classifications:Atlantic_Corridor
  rdf:type classifications:CorridorName ;
.
classifications:BILL_OF_LADING
  rdf:type classifications:DocumentType ;
.
classifications:Baltic-Adriatic_Corridor
  rdf:type classifications:CorridorName ;
.
classifications:Breakbulk
  rdf:type classifications:TransportMovementType ;
  rdfs:comment "Defines the movement of general cargo not carried in ISO standard containers." ;
  rdfs:label "break bulk" ;
.
classifications:CargoType
  rdf:type owl:Class ;
  rdfs:comment "A classification of cargo carried, or intended to be carried, on means of transport, based on its general appearance." ;
  rdfs:label "Cargo Type" ;
  rdfs:subClassOf classifications:Classifications ;
.
classifications:Classifications
  rdf:type owl:Class ;
  rdfs:comment "Various classifications of different types of e.g. cargo or container, or codelists for standards such as dangerous goods codes or nature of cargo" ;
  rdfs:label "Classifications" ;
  rdfs:subClassOf owl:Thing ;
.
classifications:ContainerType
  rdf:type owl:Class ;
  rdfs:comment "A classification of container to represent types of container according to community standards." ;
  rdfs:label "Container Type" ;
  rdfs:subClassOf classifications:Classifications ;
.
classifications:CorridorName
  rdf:type owl:Class ;
  rdfs:comment """Core network corridors were introduced to facilitate the coordinated implementation of the core network in Europe. 
Nine core network corridors are identified in the annex to the CEF Regulation, which includes a list of projects pre-identified for possible EU funding during the period 2014-2020, based on their added value for TEN-T development and their maturity status.""" ;
  rdfs:label "Corridor Name" ;
  rdfs:subClassOf classifications:Classifications ;
.
classifications:D
  rdf:type classifications:NatureOfCargo ;
  rdfs:label "Dangerous" ;
.
classifications:D_1
  rdfs:label "Reefer" ;
.
classifications:DangerousGoods
  rdf:type owl:Class ;
  rdfs:comment "A hazardous or non-hazardous substance which may pose risks to people and/or the environment for which the transportation is regulated by dangerous goods regulations." ;
  rdfs:label "Dangerous Goods" ;
  rdfs:subClassOf classifications:Classifications ;
.
classifications:DocumentType
  rdf:type owl:Class ;
  rdfs:label "Document" ;
  rdfs:subClassOf classifications:Classifications ;
.
classifications:E
  rdf:type classifications:NatureOfCargo ;
  rdfs:label "Excise" ;
.
classifications:EquipmentTypeCode
  rdf:type owl:Class ;
  rdfs:comment "an enumeration of euqipment type codes." ;
  rdfs:label "Equipment Type Code" ;
  rdfs:subClassOf classifications:Classifications ;
.
classifications:FCL-FCL
  rdf:type classifications:TransportMovementType ;
  rdfs:comment """Defines the movement of cargo packed by the shipper or
              shipper's agent and unpacked by the consignee or
              consignee's agent. 'FCL' means Full Container Load.""" ;
.
classifications:GoodsTypeCode
  rdf:type owl:Class ;
  rdfs:comment "A classification of codes that specify the different type of goods within the industry." ;
  rdfs:label "Goods Type Code" ;
  rdfs:subClassOf classifications:Classifications ;
.
classifications:LCL-LCL
  rdf:type classifications:TransportMovementType ;
  rdfs:comment """ Defines the movement of cargo packed in and unpacked
              from containers by the carrier on behalf of the
              shipper/consignee. 'LCL' means Less than Container Load.""" ;
.
classifications:LogisticsTransactionDocument
  rdf:type owl:Class ;
  rdfs:comment "A classification of the different types of documents used during logistics transactions." ;
  rdfs:label "Logistics Transaction Document" ;
  rdfs:subClassOf classifications:Classifications ;
.
classifications:Mediterranean_Corridor
  rdf:type classifications:CorridorName ;
.
classifications:NatureOfCargo
  rdf:type owl:Class ;
  rdfs:comment "A classification of codes or vocabularies that express the nature of cargo." ;
  rdfs:label "Nature of Cargo" ;
  rdfs:subClassOf classifications:Classifications ;
.
classifications:North_Sea-Baltic_Corridor
  rdf:type classifications:CorridorName ;
.
classifications:North_Sea-Mediterranean_Corridor
  rdf:type classifications:CorridorName ;
.
classifications:Orient_East-Med_Corridor
  rdf:type classifications:CorridorName ;
.
classifications:PackageType
  rdf:type owl:Class ;
  rdfs:comment """A classification of packaging materials and components used in any packaging operation to wrap, contain and protect articles or substances during transport. The shape or configuration of a package
as it appears for transport is also specified.""" ;
  rdfs:label "Package Type" ;
  rdfs:subClassOf classifications:Classifications ;
  rdfs:subClassOf [
      rdf:type owl:Restriction ;
      owl:minQualifiedCardinality "1"^^xsd:nonNegativeInteger ;
      owl:onDataRange xsd:string ;
      owl:onProperty classifications:packageCode ;
    ] ;
  rdfs:subClassOf [
      rdf:type owl:Restriction ;
      owl:minQualifiedCardinality "1"^^xsd:nonNegativeInteger ;
      owl:onDataRange xsd:string ;
      owl:onProperty classifications:packageTypeName ;
    ] ;
  rdfs:subClassOf [
      rdf:type owl:Restriction ;
      owl:minQualifiedCardinality "1"^^xsd:nonNegativeInteger ;
      owl:onDataRange xsd:string ;
      owl:onProperty classifications:packageTypeNumericCode ;
    ] ;
.
classifications:R
  rdf:type classifications:NatureOfCargo ;
  rdfs:label "Reefer" ;
.
classifications:RO-RO
  rdf:type classifications:ContainerType ;
.
classifications:Rhine-Alpine_Corridor
  rdf:type classifications:CorridorName ;
.
classifications:Rhine-Danube_Corridor
  rdf:type classifications:CorridorName ;
.
classifications:Rhine_Alpine_Corridor
  rdf:type classifications:CorridorName ;
.
classifications:Road
  rdf:type classifications:TransportModality ;
.
classifications:SEA_WAYBILL
  rdf:type classifications:DocumentType ;
.
classifications:Safety_and_hazard_data_sheet
  rdf:type classifications:LogisticsTransactionDocument ;
  rdfs:comment "A statement of an account containing the booked items as in the ledger of the account servicing financial institution." ;
  rdfs:label "Safety and hazard data sheet" ;
.
classifications:Scandinavian-Mediterranean_Corridor
  rdf:type classifications:CorridorName ;
.
classifications:Sea
  rdf:type classifications:TransportModality ;
.
classifications:SealConditionCodeType
  rdf:type owl:Class ;
  rdfs:comment "A classification of codes that specify the conditions of seals e.g. damaged or in right condition." ;
  rdfs:label "Seal Condition Code Type" ;
  rdfs:subClassOf classifications:Classifications ;
.
classifications:TransportModality
  rdf:type owl:Class ;
  rdfs:comment "A classification of the various modes used for a transportation movement. For each mode, there are several means of transport. They are: a. inland surface transportation (rail, road, and inland waterway); b. sea transport (coastal and ocean); c. air transportation; and d. pipelines. For the purpose of the usecase, we encode the top individulas only. Sea, Road, Air." ;
  rdfs:label "Transport Modality" ;
  rdfs:subClassOf classifications:Classifications ;
.
classifications:TransportMovementType
  rdf:type owl:Class ;
  rdfs:comment "A classification which specifies transport movement details for a goods item or equipment. For the purpose of this project ,we selected only few examples to demonstrate in the proof of concept -- the complete list can be found here: https://www.stylusstudio.com/edifact/D04B/8335.htm" ;
  rdfs:label "Transport Movement Type" ;
  rdfs:subClassOf classifications:Classifications ;
.
classifications:UNDGCode
  rdf:type owl:DatatypeProperty ;
  rdfs:comment "Goods can be assigned a UNDG code to identify the hazardous nature of the goods." ;
  rdfs:domain classifications:DangerousGoods ;
  rdfs:label "UNDG code" ;
  rdfs:range xsd:string ;
.
classifications:VERIFY_COPY
  rdf:type classifications:DocumentType ;
.
classifications:W
  rdf:type classifications:NatureOfCargo ;
  rdfs:label "Waste" ;
.
classifications:bulk
  rdf:type classifications:CargoType ;
  rdfs:comment "Typical examples of dry bulk transport are building materials such as sand and gravel or grain and fodder. But also wet bulk such as oil, gas and ore are examples of bulk commodities." ;
.
classifications:codeContent
  rdf:type owl:DatatypeProperty ;
  rdfs:comment "Classification of the seal code conditions type" ;
  rdfs:domain classifications:SealConditionCodeType ;
  rdfs:label "Code content" ;
  rdfs:range xsd:integer ;
.
classifications:containers
  rdf:type classifications:CargoType ;
.
classifications:dangerousGoodsClassification
  rdf:type owl:ObjectProperty ;
  rdfs:domain DigitalTwin:Goods ;
  rdfs:range classifications:DangerousGoods ;
.
classifications:dangerousGoodsRegulationCode
  rdf:type owl:DatatypeProperty ;
  rdfs:comment "Dangerous goods require a dangerous goods regulation code. The code consists of 3 characters." ;
  rdfs:domain classifications:DangerousGoods ;
  rdfs:label "Dangerous Goods Regulation Code" ;
  rdfs:range xsd:string ;
.
classifications:generalCargo
  rdf:type classifications:CargoType ;
  rdfs:comment "Contrary to mass or bulk goods, general cargo comprises materials of which the quantity is not registered per size or weight  but per individual item. General cargo is transported in boxes, crates, drums or bales. Examples of general cargo are cars, paper, kerbstone and machinery." ;
  rdfs:label "visualisation" ;
.
classifications:hazmatName
  rdf:type owl:DatatypeProperty ;
  rdfs:comment "Goods that are classified as dangerous are described in more detail using the hazardous materials UN code system. This is the corresponding name of the applicable UN code." ;
  rdfs:domain classifications:DangerousGoods ;
  rdfs:label "Dangerous Goods" ;
  rdfs:range xsd:string ;
.
classifications:hazmatUNCode
  rdf:type owl:DatatypeProperty ;
  rdfs:comment "Goods that are classified as dangerous are described in more detail using the hazardous materials UN code" ;
  rdfs:domain classifications:DangerousGoods ;
  rdfs:label "Hazmat UN code" ;
  rdfs:range xsd:string ;
.
classifications:packageCode
  rdf:type owl:DatatypeProperty ;
  rdfs:comment "Package code based on Unece Standardisations." ;
  rdfs:domain DigitalTwin:Package ;
  rdfs:label "Package Code" ;
  rdfs:range xsd:string ;
.
classifications:packageTypeName
  rdf:type owl:DatatypeProperty ;
  rdfs:comment "Package type name based on UNECE standardisations. Retrieved from internal project ProfileData postgres database." ;
  rdfs:domain classifications:PackageType ;
  rdfs:label "Package Type Name" ;
  rdfs:range xsd:string ;
.
classifications:packageTypeNumericCode
  rdf:type owl:DatatypeProperty ;
  rdfs:comment "Two digit numeric code for expressing types of package." ;
  rdfs:domain classifications:PackageType ;
  rdfs:label "Package Type Numeric Code" ;
  rdfs:range xsd:integer ;
.
classifications:pallets
  rdf:type classifications:CargoType ;
  rdfs:label "Number of TEU" ;
.
classifications:transportMovementCode
  rdf:type owl:DatatypeProperty ;
  rdfs:comment "The code of the transport movement code." ;
  rdfs:domain classifications:TransportMovementType ;
  rdfs:label "Transport Movement Code" ;
  rdfs:range xsd:string ;
.
classifications:transportMovementID
  rdf:type owl:DatatypeProperty ;
  rdfs:comment "The ID of the transport movement type." ;
  rdfs:domain classifications:TransportMovementType ;
  rdfs:label "Transport Movement Code" ;
  rdfs:range xsd:string ;
.
