# baseURI: https://ontology.tno.nl/logistics/federated/DerivedConcepts
# imports: https://ontology.tno.nl/logistics/federated/BusinessService
# imports: https://ontology.tno.nl/logistics/federated/Classifications
# imports: https://ontology.tno.nl/logistics/federated/DigitalTwin
# imports: https://ontology.tno.nl/logistics/federated/Event
# imports: https://ontology.tno.nl/logistics/federated/PhysicalInfrastructure

@prefix : <https://ontology.tno.nl/logistics/federated/DerivedConcepts> .
@prefix BusinessService: <https://ontology.tno.nl/logistics/federated/BusinessService#> .
@prefix derivedConcept: <https://ontology.tno.nl/logistics/federated/DerivedConcepts#> .
@prefix ecallUsecase: <https://ontology.tno.nl/logistics/federated/ecallUsecase#> .
@prefix owl: <http://www.w3.org/2002/07/owl#> .
@prefix rdf: <http://www.w3.org/1999/02/22-rdf-syntax-ns#> .
@prefix rdfs: <http://www.w3.org/2000/01/rdf-schema#> .
@prefix sh: <http://www.w3.org/ns/shacl#> .
@prefix skos: <http://www.w3.org/2004/02/skos/core#> .
@prefix xsd: <http://www.w3.org/2001/XMLSchema#> .
@prefix dc: <http://purl.org/dc/elements/1.1/> .
@prefix dcterms: <http://purl.org/dc/terms/> .

<https://ontology.tno.nl/logistics/federated/DerivedConcepts>
  rdf:type owl:Ontology ;
  owl:imports <https://ontology.tno.nl/logistics/federated/BusinessService> ;
  owl:imports <https://ontology.tno.nl/logistics/federated/Classifications> ;
  owl:imports <https://ontology.tno.nl/logistics/federated/DigitalTwin> ;
  owl:imports <https://ontology.tno.nl/logistics/federated/Event> ;
  owl:imports <https://ontology.tno.nl/logistics/federated/PhysicalInfrastructure> ;
  dc:creator "Dena Tahvildari, Cornelis Bouter, Maaike Burghoorn";
  owl:versionInfo "Created with TopBraid Composer" ;
  dcterms:description """This ontology contains classes, attributes, relation about 
  						 from Derived Concepts relevant in the
  						 FEDeRATED ontology domain. The concepts in this ontology
  						 are intended to be inferred through reasoning rules or
  						 queries instead of directly instantiated.""" ;
  dcterms:isRequiredBy  <https://ontology.tno.nl/logistics/federated/DigitalTwin> ,
    					<https://ontology.tno.nl/logistics/federated/BusinessService> ,
    					<https://ontology.tno.nl/logistics/federated/PhysicalInfrastructure> ;
  dcterms:requires 		<https://ontology.tno.nl/logistics/federated/DigitalTwin> ,
    					<https://ontology.tno.nl/logistics/federated/BusinessService> ,
    					<https://ontology.tno.nl/logistics/federated/PhysicalInfrastructure> ;
  dcterms:language "en" ;
  owl:versionIRI <https://ontology.tno.nl/logistics/federated/DerivedConceptsv-0.1>;
  dcterms:issued "2021-03-15"^^xsd:DateTime ;
  dcterms:created "2021-02-11"^^xsd:DateTime ;
.
derivedConcept:CargoTrack
  rdf:type owl:Class ;
  rdf:type sh:NodeShape ;
  rdfs:subClassOf derivedConcept:Track ;
.
derivedConcept:Consignment
  rdf:type owl:Class ;
  rdf:type sh:NodeShape ;
  rdfs:comment "A consignment is a business transaction of a shipper as customer with a service provider (e.g. a carrier or forwarder) for the transport of goods or containers from one location to another, where all goods and containers have to arrive in a given time period. The time period indicates that the goods or containers can arrive with different transport means at different times, but they all have to present after the period has ended." ;
  rdfs:subClassOf owl:Thing ;
  rdfs:subClassOf [
      rdf:type owl:Restriction ;
      owl:minQualifiedCardinality "1"^^xsd:nonNegativeInteger ;
      owl:onClass BusinessService:BusinessTransaction ;
      owl:onProperty derivedConcept:involves ;
    ] ;
  rdfs:subClassOf [
      rdf:type owl:Restriction ;
      owl:minQualifiedCardinality "1"^^xsd:nonNegativeInteger ;
      owl:onClass BusinessService:TransportService ;
      owl:onProperty derivedConcept:involves ;
    ] ;
  rdfs:subClassOf [
      rdf:type owl:Restriction ;
      owl:minQualifiedCardinality "1"^^xsd:nonNegativeInteger ;
      owl:onClass BusinessService:logisticsActor ;
      owl:onProperty derivedConcept:involves ;
    ] ;
  rdfs:subClassOf [
      rdf:type owl:Restriction ;
      owl:minQualifiedCardinality "1"^^xsd:nonNegativeInteger ;
      owl:onClass <https://ontology.tno.nl/logistics/federated/LogisticsRoles#ServiceProvider> ;
      owl:onProperty derivedConcept:involves ;
    ] ;
  rdfs:subClassOf [
      rdf:type owl:Restriction ;
      owl:minQualifiedCardinality "1"^^xsd:nonNegativeInteger ;
      owl:onClass <https://ontology.tno.nl/logistics/federated/PhysicalInfrastructure#Location> ;
      owl:onProperty derivedConcept:involves ;
    ] ;
.
derivedConcept:ContainerTrack
  rdf:type owl:Class ;
  rdf:type sh:NodeShape ;
  rdfs:comment "timed sequence of transport legs for a particular container. A container track can be derived from data provided by the individual transport legs." ;
  rdfs:subClassOf derivedConcept:Track ;
.
derivedConcept:GoodTrack
  rdf:type owl:Class ;
  rdf:type sh:NodeShape ;
  rdfs:comment "timed sequence of transport legs and/or container tracks relevant for goods." ;
  rdfs:subClassOf derivedConcept:Track ;
.
derivedConcept:GoodsFlow
  rdf:type owl:Class ;
  rdf:type sh:NodeShape ;
  rdfs:comment "Cargo flow in terms of origin, transshipment locations, destination and transport legs" ;
  rdfs:subClassOf owl:Thing ;
.
derivedConcept:Itinerary
  rdf:type owl:Class ;
  rdf:type sh:NodeShape ;
  rdfs:comment "a timed sequence of transshipment locations or hubs passed by a transport means to load and/or discharge cargo. An itinerary, or voyage of a vessel, is expressed in data properties and associations of the semantic model." ;
  rdfs:subClassOf owl:Thing ;
  skos:altLabel "Voyage" ;
.
derivedConcept:LocatedAt
  rdf:type owl:ObjectProperty ;
.
derivedConcept:Rout
  rdf:type owl:Class ;
  rdf:type sh:NodeShape ;
  rdfs:comment "the use of the infrastructure (sea, road, rail, etc.) taken by a transport means between any two locations of its itinerary. A route is also expressed as in data properties and associations of the semantic model. " ;
  rdfs:subClassOf owl:Thing ;
.
derivedConcept:Shipment
  rdf:type owl:Class ;
  rdf:type sh:NodeShape ;
  rdfs:comment "A shipment is a business transaction with a carrier for the transport of goods or containers from one location to another, where all goods and containers have to arrive in a given time period. This is similar to a consignment; however, it is always a carrier acting as service provider." ;
  rdfs:subClassOf owl:Thing ;
  rdfs:subClassOf [
      rdf:type owl:Restriction ;
      owl:minQualifiedCardinality "1"^^xsd:nonNegativeInteger ;
      owl:onClass derivedConcept:Consignment ;
      owl:onProperty derivedConcept:contains ;
    ] ;
.
derivedConcept:Track
  rdf:type owl:Class ;
  rdf:type sh:NodeShape ;
  rdfs:comment "Abstract Class for grouping different types of tracks  such as cargo track, container track." ;
  rdfs:subClassOf owl:Thing ;
  rdfs:subClassOf [
      rdf:type owl:Restriction ;
      owl:minQualifiedCardinality "1"^^xsd:nonNegativeInteger ;
      owl:onClass <https://ontology.tno.nl/logistics/federated/PhysicalInfrastructure#Location> ;
      owl:onProperty derivedConcept:LocatedAt ;
    ] ;
.
derivedConcept:TransportFlow
  rdf:type owl:Class ;
  rdf:type sh:NodeShape ;
  rdfs:comment "The activities and movement of a transport means (i.e. vessel) as a basis for anomaly detection" ;
  rdfs:subClassOf owl:Thing ;
.
derivedConcept:TransportLeg
  rdf:type owl:Class ;
  rdf:type sh:NodeShape ;
  rdfs:comment "transport of particular cargo between two adjacent (in time) locations with only one transport means (e.g. POL-POD; this refers to roles of locations like POL – Port of Loading – and POD – Port of Discharge (see note on roles))." ;
  rdfs:subClassOf owl:Thing ;
.
derivedConcept:TruckItinerary
  rdf:type owl:Class ;
  rdf:type sh:NodeShape ;
  rdfs:comment "truck itinerary has synonym ‘trip" ;
  rdfs:subClassOf derivedConcept:Itinerary ;
  skos:altLabel "trip" ;
.
derivedConcept:contains
  rdf:type owl:ObjectProperty ;
.
derivedConcept:involves
  rdf:type owl:ObjectProperty ;
.
