# baseURI: https://ontology.tno.nl/logistics/federated/Event
# imports: https://ontology.tno.nl/logistics/federated/BusinessService
# imports: https://ontology.tno.nl/logistics/federated/Classifications
# imports: https://ontology.tno.nl/logistics/federated/DigitalTwin
# imports: https://ontology.tno.nl/logistics/federated/PhysicalInfrastructure
# imports: https://ontology.tno.nl/logistics/federated/ReusableTags
# prefix: Event

@prefix : <https://ontology.tno.nl/logistics/federated/Event#> .
@prefix DigitalTwin: <https://ontology.tno.nl/logistics/federated/DigitalTwin#> .
@prefix Event: <https://ontology.tno.nl/logistics/federated/Event#> .
@prefix businessService: <https://ontology.tno.nl/logistics/federated/BusinessService#> .
@prefix dc: <http://purl.org/dc/elements/1.1/> .
@prefix dcterms: <http://purl.org/dc/terms/> .
@prefix owl: <http://www.w3.org/2002/07/owl#> .
@prefix pi: <https://ontology.tno.nl/logistics/federated/PhysicalInfrastructure#> .
@prefix rdf: <http://www.w3.org/1999/02/22-rdf-syntax-ns#> .
@prefix rdfs: <http://www.w3.org/2000/01/rdf-schema#> .
@prefix xsd: <http://www.w3.org/2001/XMLSchema#> .

<https://ontology.tno.nl/logistics/federated/Event>
  rdf:type owl:Ontology ;
  dc:creator "Dena Tahvildari, Maaike Burghoorn, Cornelis Bouter" ;
  dcterms:created "2020-07-17" ;
  dcterms:description "This ontology contains classes, attributes, relation about logistic Events." ;
  dcterms:issued "2021-03-15" ;
  dcterms:language "en" ;
  dcterms:requires <https://ontology.tno.nl/logistics/federated/BusinessService> ;
  dcterms:requires <https://ontology.tno.nl/logistics/federated/DigitalTwin> ;
  dcterms:requires <https://ontology.tno.nl/logistics/federated/PhysicalInfrastructure> ;
  owl:imports <https://ontology.tno.nl/logistics/federated/BusinessService> ;
  owl:imports <https://ontology.tno.nl/logistics/federated/Classifications> ;
  owl:imports <https://ontology.tno.nl/logistics/federated/DigitalTwin> ;
  owl:imports <https://ontology.tno.nl/logistics/federated/PhysicalInfrastructure> ;
  owl:imports <https://ontology.tno.nl/logistics/federated/ReusableTags> ;
  owl:versionIRI <https://ontology.tno.nl/logistics/federated/Eventv-0.1> ;
.
Event:ATAEvent
  rdf:type owl:Class ;
  rdfs:comment "The Actual Time of Arrival event is an ArrivalEvent with an actual time." ;
  rdfs:label "Actual date/time of arrival (ATA)" ;
  rdfs:subClassOf Event:ArrivalEvent ;
.
Event:ATDEvent
  rdf:type owl:Class ;
  rdfs:comment "An ATD Event (Actual Time of Departure Event) is a departure event with the actual date-time." ;
  rdfs:label "ActualTimeOfDepartureEvent" ;
  rdfs:subClassOf Event:DepartureEvent ;
.
Event:Actual
  rdf:type Event:DateTimeType ;
  rdfs:label "Actual" ;
.
Event:ArrivalEvent
  rdf:type owl:Class ;
  rdfs:comment "An Arrival Event is an association between a Digital Twin type TransportMeans and a location. It should have milestone Start." ;
  rdfs:label "Arrival Event" ;
  rdfs:subClassOf Event:Event ;
.
Event:BulkDischarge
  rdf:type owl:Class ;
  rdfs:label "Has Manager" ;
  rdfs:subClassOf Event:BulkTransportEvent ;
  rdfs:subClassOf Event:DischargeEvent ;
.
Event:BulkLoadEvent
  rdf:type owl:Class ;
  rdfs:label "Has Manager" ;
  rdfs:subClassOf Event:BulkTransportEvent ;
  rdfs:subClassOf Event:LoadEvent ;
.
Event:BulkTransportEvent
  rdf:type owl:Class ;
  rdfs:label "Has Manager" ;
  rdfs:subClassOf Event:CargoEvent ;
.
Event:CargoEvent
  rdf:type owl:Class ;
  rdfs:comment "A Cargo event is any event that associates goods, equipment or bulk products with the Digital Twin that transports it." ;
  rdfs:label "Cargo Event" ;
  rdfs:subClassOf Event:Event ;
.
Event:ContainerDischargeEvent
  rdf:type owl:Class ;
  rdfs:comment "In a Container Discharge Event an equipment of type Container is discharged from its transportation means." ;
  rdfs:label "Container Discharge Event" ;
  rdfs:subClassOf Event:DischargeEvent ;
  rdfs:subClassOf Event:EquipmentTransportEvent ;
.
Event:ContainerLoadEvent
  rdf:type owl:Class ;
  rdfs:comment "With a Container Load Event an association between an equipment of type Container and a transport means is established, because the container is loaded on some transport means." ;
  rdfs:label "Container Load Event" ;
  rdfs:subClassOf Event:EquipmentLoadEvent ;
.
Event:DateTimeType
  rdf:type owl:Class ;
  rdfs:comment "This concept contains the various types of date that an event may have an association to: actual, estimated, expected, planned, and requested. These are all modelled as instances of this type." ;
  rdfs:domain Event:Event ;
  rdfs:label "Date Time Type" ;
  rdfs:subClassOf owl:Thing ;
.
Event:DepartureEvent
  rdf:type owl:Class ;
  rdfs:comment "A Departure Event is an association between a Digital Twin type TransportMeans and a Location. It should have milestone End." ;
  rdfs:label "Departure Event" ;
  rdfs:subClassOf Event:Event ;
.
Event:DischargeEvent
  rdf:type owl:Class ;
  rdfs:subClassOf Event:CargoEvent ;
.
Event:DropOffEvent
  rdf:type owl:Class ;
  rdfs:comment "An Event for dropping off a piece of equipment at a particular location." ;
  rdfs:label "Drop Off Event" ;
  rdfs:subClassOf Event:Event ;
.
Event:DropOffTimeWindowEvent
  rdf:type owl:Class ;
  rdfs:comment "An event to cover the intended time window during which some cargo may be dropped off. So, an association between a time interval and an equipment." ;
  rdfs:label "Drop Off Time Window Event" ;
  rdfs:subClassOf Event:Event ;
.
Event:ETAEvent
  rdf:type owl:Class ;
  rdfs:comment "An Estimated Time of Arrival Event is an ArrivalEvent with an estimated date-time." ;
  rdfs:label "Estimated Time of Arrival Event" ;
  rdfs:subClassOf Event:ArrivalEvent ;
.
Event:ETDEvent
  rdf:type owl:Class ;
  rdfs:comment "An ETD event (Estimated Time of Departure Event) is a DepartureEvent with an estimated date-time." ;
  rdfs:label "Estimated Time of Departure Event" ;
  rdfs:subClassOf Event:DepartureEvent ;
.
Event:End
  rdf:type Event:Milestone ;
  rdfs:label "End" ;
.
Event:EquipmentLoadEvent
  rdf:type owl:Class ;
  rdfs:comment "With a Cargo Load Event an association between equipment and transport means is established, because the equipment is loaded on the transport means." ;
  rdfs:label "Cargo Load Event" ;
  rdfs:subClassOf Event:EquipmentTransportEvent ;
  rdfs:subClassOf Event:LoadEvent ;
.
Event:EquipmentTransportEvent
  rdf:type owl:Class ;
  rdfs:comment "In a Cargo Discharge Event the connection between equipment and transport means is released, since the equipment is discharged off the transport means." ;
  rdfs:label "Cargo Discharge Event" ;
  rdfs:subClassOf Event:CargoEvent ;
.
Event:Estimated
  rdf:type Event:DateTimeType ;
  rdfs:label "Estimated" ;
.
Event:Event
  rdf:type owl:Class ;
  rdfs:comment """An event reflects any physical activity in the real world, creating, updating, or 'deleting' an association between physical objects or entities. There are many synomyms based on combinations of entities, date/time, and physical activities. 				
""" ;
  rdfs:label "Event" ;
  rdfs:subClassOf [
      rdf:type owl:Restriction ;
      owl:minCardinality "1"^^xsd:nonNegativeInteger ;
      owl:onProperty Event:DateTimeType ;
    ] ;
  rdfs:subClassOf [
      rdf:type owl:Restriction ;
      owl:minCardinality "1"^^xsd:nonNegativeInteger ;
      owl:onProperty Event:DigitalTwin_detail ;
    ] ;
.
Event:Expected
  rdf:type Event:DateTimeType ;
  rdfs:label "Expected" ;
.
Event:GoodsDischargeEvent
  rdf:type owl:Class ;
  rdfs:label "Has Manager" ;
  rdfs:subClassOf Event:DischargeEvent ;
  rdfs:subClassOf Event:GoodsTransportEvent ;
.
Event:GoodsEquipmentEvent
  rdf:type owl:Class ;
  rdfs:comment "A Goods Equipment Event establishes the association between a goods or packaged product and an equipment." ;
  rdfs:label "Goods Equipment Event" ;
  rdfs:subClassOf Event:CargoEvent ;
.
Event:GoodsLoadEvent
  rdf:type owl:Class ;
  rdfs:comment "Association Transport Means - Goods. Load goods without intermediate equipment." ;
  rdfs:label "Has Manager" ;
  rdfs:subClassOf Event:GoodsTransportEvent ;
  rdfs:subClassOf Event:LoadEvent ;
.
Event:GoodsStructuringEvent
  rdf:type owl:Class ;
  rdfs:comment "Events forming an association between two transportable objects (i.e., products or goods)." ;
  rdfs:label "Transportable Object Event" ;
  rdfs:subClassOf Event:Event ;
.
Event:GoodsTransportEvent
  rdf:type owl:Class ;
  rdfs:label "Has Manager" ;
  rdfs:subClassOf Event:CargoEvent ;
.
Event:LoadEvent
  rdf:type owl:Class ;
  rdfs:subClassOf Event:CargoEvent ;
.
Event:MergeEvent
  rdf:type owl:Class ;
  rdfs:comment "Merge two sets of goods into a single combined set of goods. This Event contains an association meaning that the association with lesser volume is merged into the association with the higher volume. We expect the association with the higher volume to have several Merge Events associated with it, the sum of which is equal to the volume of that association." ;
  rdfs:label "Merge Event" ;
  rdfs:subClassOf Event:GoodsStructuringEvent ;
.
Event:Milestone
  rdf:type owl:Class ;
  rdfs:comment "Each Event should have a Milestone associated with it. At the moment, only Start and End are allowed milestones. All allowed Milestone should be of this type." ;
  rdfs:subClassOf owl:Thing ;
.
Event:PackagingEvent
  rdf:type owl:Class ;
  rdfs:comment "An event assocation between transportable objects (Goods or Products) to show that one has been packaged into the other." ;
  rdfs:label "Packaging Event" ;
  rdfs:subClassOf Event:GoodsStructuringEvent ;
.
Event:PickupEvent
  rdf:type owl:Class ;
  rdfs:label "Pick Up Event" ;
  rdfs:subClassOf Event:Event ;
.
Event:PickupTimeWindowEvent
  rdf:type owl:Class ;
  rdfs:comment "Event for the time window between which a piece of equipment may be picked up." ;
  rdfs:label "Pick Up Time Window Event" ;
  rdfs:subClassOf Event:Event ;
.
Event:Planned
  rdf:type Event:DateTimeType ;
  rdfs:label "Planned" ;
.
Event:PushBargeLoadEvent
  rdf:type owl:Class ;
  rdfs:comment "An association between an equipment of type PushBarge and a transport means of type Ship is established via this event. The push barge is connected to the ship pushing it forward." ;
  rdfs:label "Push Barge Load Event" ;
  rdfs:subClassOf Event:EquipmentLoadEvent ;
.
Event:RailwayWagonLoadEvent
  rdf:type owl:Class ;
  rdfs:comment "With the Railway Wagon Load Event a railway wagon is an association between an equipment and a railway wagon." ;
  rdfs:label "Railway Wagon Load Event" ;
  rdfs:subClassOf Event:EquipmentLoadEvent ;
.
Event:SplitEvent
  rdf:type owl:Class ;
  rdfs:comment "Split a set of transportable object into smaller sets of transportable object." ;
  rdfs:label "Split Event" ;
  rdfs:subClassOf Event:GoodsStructuringEvent ;
.
Event:Start
  rdf:type Event:Milestone ;
  rdfs:label "Start" ;
.
Event:StripEvent
  rdf:type owl:Class ;
  rdfs:comment "Association to unload a piece of equipment with goods." ;
  rdfs:label "Strip" ;
  rdfs:subClassOf Event:GoodsEquipmentEvent ;
.
Event:StuffEvent
  rdf:type owl:Class ;
  rdfs:comment "Association to load a piece of equipment with goods or packaged products." ;
  rdfs:label "Stuff Event" ;
  rdfs:subClassOf Event:GoodsEquipmentEvent ;
.
Event:UnpackEvent
  rdf:type owl:Class ;
  rdfs:comment "An unpack event means that goods/packaged products are unpacked into another packaging type of the goods/packaged products." ;
  rdfs:label "Unpack Event" ;
  rdfs:subClassOf Event:GoodsStructuringEvent ;
.
Event:end
  rdf:type Event:MileStone ;
.
Event:expectedDropOffDate
  rdf:type owl:DatatypeProperty ;
  rdfs:range xsd:date ;
.
Event:expectedDropoffTime_Earliest
  rdf:type owl:DatatypeProperty ;
  rdfs:range xsd:dateTime ;
.
Event:expectedDropoffTime_Latest
  rdf:type owl:DatatypeProperty ;
  rdfs:range xsd:dateTime ;
.
Event:expectedPickupDate
  rdf:type owl:DatatypeProperty ;
  rdfs:domain Event:PickupEvent ;
  rdfs:range xsd:date ;
.
Event:expectedPickupTime_Earliest
  rdf:type owl:DatatypeProperty ;
  rdfs:domain Event:PickupEvent ;
  rdfs:range xsd:dateTime ;
.
Event:expectedPickupTime_Latest
  rdf:type owl:DatatypeProperty ;
  rdfs:domain Event:PickupEvent ;
  rdfs:range xsd:dateTime ;
.
Event:hasDateTimeType
  rdf:type owl:ObjectProperty ;
  rdfs:comment "This property relates an Event with a datetime to the individual that represents whether the datetime is the actual, estimated, expected, planned, or requested datetime." ;
  rdfs:domain Event:Event ;
  rdfs:label "Has DateTime Type" ;
  rdfs:range Event:DateTimeType ;
  rdfs:seeAlso Event:hasTimestamp ;
.
Event:hasDropOffTime
  rdf:type owl:DatatypeProperty ;
  rdfs:domain Event:Event ;
  rdfs:label "Has Pickup Time" ;
  rdfs:range xsd:dateTime ;
.
Event:hasMilestone
  rdf:type owl:ObjectProperty ;
  rdfs:comment "This property relates an Event to its Milestone, which can be either Start or End." ;
  rdfs:domain Event:Event ;
  rdfs:label "has Milestone" ;
  rdfs:range Event:Milestone ;
.
Event:hasPickupTime
  rdf:type owl:DatatypeProperty ;
  rdfs:domain Event:Event ;
  rdfs:label "Has Pickup Time" ;
  rdfs:range xsd:dateTime ;
.
Event:hasTimestamp
  rdf:type owl:DatatypeProperty ;
  rdfs:comment "This property relates an Event to the timestamp associated with it. A timestamp modifier can be entered via hasDateTimeType." ;
  rdfs:domain Event:Event ;
  rdfs:label "Has Timestamp" ;
  rdfs:range xsd:dateTime ;
  rdfs:seeAlso Event:hasDateTimeType ;
.
Event:involves
  rdf:type owl:ObjectProperty ;
  rdfs:comment "An Event has two associations established with Digital Twins, Business Transactions, Locations or Logistic Actors. These two associations as formed via (subproperties of) the Event:involves object property. This meaning of this association depends on the particular subproperty being used. The subtype of Event is inferred based on the subproperties used." ;
  rdfs:domain Event:Event ;
  rdfs:label "Involves" ;
  rdfs:range owl:Thing ;
.
Event:involvesBusinessTransaction
  rdf:type owl:ObjectProperty ;
  rdfs:comment "This relation establishes an association between an Event and a Business Transaction. The exact meaning depends on the type of Event, which is inferred from this property and the second association the event has." ;
  rdfs:domain Event:Event ;
  rdfs:label "Involves Business Transaction" ;
  rdfs:range businessService:BusinessTransaction ;
  rdfs:subPropertyOf Event:involves ;
.
Event:involvesDigitalTwin
  rdf:type owl:ObjectProperty ;
  rdfs:comment "This relation establishes an association between an Event and a Digital Twin. The exact meaning depends on the type of Event, which is inferred from this property and the second association the event has." ;
  rdfs:domain Event:Event ;
  rdfs:label "Involves Digital Twin" ;
  rdfs:range DigitalTwin:PhysicalObject ;
  rdfs:subPropertyOf Event:involves ;
.
Event:involvesLogisticsActor
  rdf:type owl:ObjectProperty ;
  rdfs:comment "This relation establishes an association between an Event and a Logistics Actor. The exact meaning depends on the type of Event, which is inferred from this property and the second association the event has." ;
  rdfs:domain Event:Event ;
  rdfs:label "Involves Logistics Actor" ;
  rdfs:range businessService:LegalPerson ;
  rdfs:subPropertyOf Event:involves ;
.
Event:involvesPhysicalInfrastructure
  rdf:type owl:ObjectProperty ;
  rdfs:comment "This relation establishes an association between an Event and a Location. The exact meaning depends on the type of Event, which is inferred from this property and the second association the event has." ;
  rdfs:domain Event:Event ;
  rdfs:label "Involves Location" ;
  rdfs:range pi:Location ;
  rdfs:subPropertyOf Event:involves ;
.
Event:start
  rdf:type Event:MileStone ;
.
