# baseURI: https://ontology.tno.nl/logistics/federated/PhysicalInfrastructure
# imports: http://www.w3.org/2003/01/geo/wgs84_pos
# prefix: pi

@prefix : <https://ontology.tno.nl/logistics/federated/PhysicalInfrastructure#> .
@prefix BusinessService: <https://ontology.tno.nl/logistics/federated/BusinessService#> .
@prefix classifications: <https://ontology.tno.nl/logistics/federated/Classifications#> .
@prefix dc: <http://purl.org/dc/elements/1.1/> .
@prefix dcterms: <http://purl.org/dc/terms/> .
@prefix owl: <http://www.w3.org/2002/07/owl#> .
@prefix pi: <https://ontology.tno.nl/logistics/federated/PhysicalInfrastructure#> .
@prefix rdf: <http://www.w3.org/1999/02/22-rdf-syntax-ns#> .
@prefix rdfs: <http://www.w3.org/2000/01/rdf-schema#> .
@prefix sh: <http://www.w3.org/ns/shacl#> .
@prefix skos: <http://www.w3.org/2004/02/skos/core#> .
@prefix xsd: <http://www.w3.org/2001/XMLSchema#> .

<https://ontology.tno.nl/logistics/federated/PhysicalInfrastructure>
  a owl:Ontology ;
  dc:creator "Dena Tahvildari, Maaike Burghoorn, Cornelis Bouter" ;
  dcterms:created "2020-07-17" ;
  dcterms:description "This ontology contains classes, attributes, relation about physical infrastructure objects that are used in Logistics Events." ;
  dcterms:isRequiredBy <https://ontology.tno.nl/logistics/federated/Event> ;
  dcterms:issued "2021-03-15" ;
  dcterms:language "en" ;
  dcterms:requires <https://ontology.tno.nl/logistics/federated/Classifications> ;
  owl:imports <http://www.w3.org/2003/01/geo/wgs84_pos> ;
  owl:versionIRI <https://ontology.tno.nl/logistics/federated/PhysicalInfrastructurev-0.1> ;
.
pi:Address
  a owl:Class ;
  rdfs:comment "The address of a location." ;
  rdfs:label "Address" ;
  rdfs:subClassOf pi:Location ;
  rdfs:subClassOf [
      a owl:Restriction ;
      owl:minQualifiedCardinality "1"^^xsd:nonNegativeInteger ;
      owl:onDataRange xsd:string ;
      owl:onProperty pi:StreetName ;
    ] ;
  rdfs:subClassOf [
      a owl:Restriction ;
      owl:minQualifiedCardinality "1"^^xsd:nonNegativeInteger ;
      owl:onDataRange xsd:string ;
      owl:onProperty pi:BuildingNumber ;
    ] ;
.
pi:Airport
  a owl:Class ;
  rdfs:comment "Location where airplanes pick or drop off freight." ;
  rdfs:label "Airport" ;
  rdfs:subClassOf pi:LogisticalFunction ;
.
pi:Anchorage
  a owl:Class ;
  rdfs:comment "A location where a ship can 'park'." ;
  rdfs:label "Anchorage" ;
  rdfs:subClassOf pi:LogisticalFunction ;
.
pi:BargeTerminal
  a owl:Class ;
  rdfs:comment "A terminal with main modality waterways where cargo of barges can be loaded/discharged." ;
  rdfs:label "Barge Terminal" ;
  rdfs:subClassOf pi:LogisticalFunction ;
.
pi:Bridge
  a owl:Class ;
  rdfs:comment "A road crossing water." ;
  rdfs:label "Bridge" ;
  rdfs:subClassOf pi:InfrastructuralObject ;
.
pi:City
  a owl:Class ;
  rdfs:comment "A city is one of the various subtypes of Location." ;
  rdfs:label "City" ;
  rdfs:subClassOf pi:Location ;
  rdfs:subClassOf [
      a owl:Restriction ;
      owl:minQualifiedCardinality "1"^^xsd:nonNegativeInteger ;
      owl:onDataRange xsd:string ;
      owl:onProperty pi:cityLoCode ;
    ] ;
  rdfs:subClassOf [
      a owl:Restriction ;
      owl:minQualifiedCardinality "1"^^xsd:nonNegativeInteger ;
      owl:onDataRange xsd:string ;
      owl:onProperty pi:postalCode ;
    ] ;
.
pi:Corridor
  a owl:Class ;
  rdfs:comment "A logistic corridor is a generalised route. It may consist of several modalities. For example, the route between Europoort and Northern Italy is a corridor, since it's a comman and important route." ;
  rdfs:label "Corridor" ;
  rdfs:subClassOf pi:Trajectory ;
.
pi:Country
  a owl:Class ;
  rdfs:comment "A Country is a geographic division with national borders." ;
  rdfs:label "Country" ;
  rdfs:subClassOf pi:Location ;
  rdfs:subClassOf [
      a owl:Restriction ;
      owl:minQualifiedCardinality "1"^^xsd:nonNegativeInteger ;
      owl:onDataRange xsd:string ;
      owl:onProperty pi:countryISOCode ;
    ] ;
  rdfs:subClassOf [
      a owl:Restriction ;
      owl:minQualifiedCardinality "1"^^xsd:nonNegativeInteger ;
      owl:onDataRange xsd:string ;
      owl:onProperty pi:countryName ;
    ] ;
.
pi:Gate
  a owl:Class ;
  rdfs:comment "An interface between road and air." ;
  rdfs:label "Gate" ;
  rdfs:subClassOf pi:LogisticalInterface ;
.
pi:Hub
  a owl:Class ;
  rdfs:comment "A place where cargo is exchanged between vehicles or/and between transport modes." ;
  rdfs:label "Hub" ;
  rdfs:subClassOf pi:LogisticalFunction ;
.
pi:InfrastructuralFunction
  a owl:Class ;
  rdfs:comment "Any part of an infrastructure used for performing logistical activities." ;
  rdfs:label "Infrastructural Function" ;
  rdfs:subClassOf <http://www.w3.org/2003/01/geo/wgs84_pos#SpatialThing> ;
  owl:disjointWith pi:LogisticalFunction ;
.
pi:InfrastructuralObject
  a owl:Class ;
  rdfs:comment "Any element in an infrastructure that might cause for a delay (e.g. bridge, lock)." ;
  rdfs:label "Infrastructural Object" ;
  rdfs:subClassOf pi:InfrastructuralFunction ;
.
pi:InfrastructuralFunctionProperty
  a owl:DatatypeProperty ;
  rdfs:comment "A super property for all properties related to infrastructural functions. -- Abstract property, do not instantiate." ;
  rdfs:label "Infrastructural Function Property" ;
.
pi:InlandTerminal
  a owl:Class ;
  rdfs:comment "An Inland Terminal can have an interface with more than one modality like inland waterways, rail and/or road (note: there are also inland terminals that have only road as modality (e.g. Interporto Bologna) or road and rail (e.g. Zaragoza Logistics Center)." ;
  rdfs:label "Inland Terminal" ;
  rdfs:subClassOf pi:LogisticalFunction ;
.
pi:Landmark
  a owl:Class ;
  rdfs:comment "A Land Mark is a an object or feature of a landscape or town that is easily recognised from a distance." ;
  rdfs:label "Land Mark" ;
  rdfs:subClassOf pi:Location ;
.
pi:Lat
  a owl:DatatypeProperty ;
  rdfs:comment "This property specifies the latitude of a specific location." ;
  rdfs:domain pi:Location ;
  rdfs:label "Latitude" ;
  rdfs:range xsd:decimal ;
  rdfs:subPropertyOf pi:LocationCoordinate ;
.
pi:Location
  a owl:Class ;
  rdfs:comment "A geographical location where several objects with various logistical functions may be." ;
  rdfs:label "Location" ;
  rdfs:subClassOf <http://www.w3.org/2003/01/geo/wgs84_pos#SpatialThing> ;
  rdfs:subClassOf <https://schema.org/Place> ;
  rdfs:subClassOf [
      a owl:Restriction ;
      owl:minQualifiedCardinality "1"^^xsd:nonNegativeInteger ;
      owl:onDataRange xsd:decimal ;
      owl:onProperty pi:Lat ;
    ] ;
  rdfs:subClassOf [
      a owl:Restriction ;
      owl:minQualifiedCardinality "1"^^xsd:nonNegativeInteger ;
      owl:onDataRange xsd:decimal ;
      owl:onProperty pi:Long ;
    ] ;
.
pi:LocationCoordinate
  a owl:DatatypeProperty ;
  rdfs:comment "The subproperties of this property specify the location coordinates of a specific location." ;
  rdfs:domain pi:Location ;
  rdfs:label "Location Coordinate" ;
  rdfs:range xsd:decimal ;
.
pi:LogisticalFunction
  a owl:Class ;
  rdfs:comment "Any location where a logistical activity is performed. A single location may have several logistical functions." ;
  rdfs:label "Logistical Function" ;
  rdfs:subClassOf <http://www.w3.org/2003/01/geo/wgs84_pos#SpatialThing> ;
.
pi:LogisticalInterface
  a owl:Class ;
  rdfs:comment "An interface where the modality of a transport may change." ;
  rdfs:label "Logistical Interface" ;
  rdfs:subClassOf <http://www.w3.org/2003/01/geo/wgs84_pos#SpatialThing> ;
.
pi:LogisticalInterfaceProperty
  a owl:DatatypeProperty ;
  rdfs:comment "A datatype property for a logistical interface. -- Abstract property, do not instantiate." ;
  rdfs:label "Logistical Interface Property" ;
.
pi:Long
  a owl:DatatypeProperty ;
  rdfs:comment "This property specifies the longitude of a specific location." ;
  rdfs:domain pi:Location ;
  rdfs:label "Longitude" ;
  rdfs:range xsd:decimal ;
  rdfs:subPropertyOf pi:LocationCoordinate ;
.
pi:Platform
  a owl:Class ;
  rdfs:comment "An interface to or from the Railway modality." ;
  rdfs:label "Platform" ;
  rdfs:subClassOf pi:LogisticalInterface ;
.
pi:Port
  a owl:Class ;
  rdfs:comment "Location where vessels pick or drop off freight." ;
  rdfs:label "Port" ;
  rdfs:subClassOf pi:LogisticalFunction ;
.
pi:Quay
  a owl:Class ;
  rdfs:comment "An interface to or from sea and inland waterways." ;
  rdfs:label "Quay" ;
  rdfs:subClassOf pi:LogisticalInterface ;
.
pi:RailwayLine
  a owl:Class ;
  rdfs:comment "A trajectory with modality 'rail'." ;
  rdfs:label "Railway Line" ;
  rdfs:subClassOf pi:Trajectory ;
.
pi:RailwayStation
  a owl:Class ;
  rdfs:comment "A location where railway wagons and locomotives drop off or pick up freight." ;
  rdfs:label "Railway Station" ;
  rdfs:subClassOf pi:InlandTerminal ;
.
pi:RailwayTerminal
  a owl:Class ;
  rdfs:comment "An inland terminal managed by a railway infrastructure manager with main modality rail." ;
  rdfs:label "Railway Terminal" ;
  rdfs:subClassOf pi:InlandTerminal ;
.
pi:Road
  a owl:Class ;
  rdfs:comment "A trajectory with modality 'road'." ;
  rdfs:label "Road" ;
  rdfs:subClassOf pi:Trajectory ;
.
pi:Terminal
  a owl:Class ;
  rdfs:comment "A location interfacing with main modality sea." ;
  rdfs:label "Terminal" ;
  rdfs:subClassOf pi:Hub ;
.
pi:Trajectory
  a owl:Class ;
  rdfs:comment "Any part of an infrastructure identified by its infrastructure manager." ;
  rdfs:label "Trajectory" ;
  rdfs:subClassOf <http://www.w3.org/2003/01/geo/wgs84_pos#SpatialThing> ;
.
pi:TrajectoryProperty
  a owl:DatatypeProperty ;
  rdfs:comment "DO NOT Instantiate -- superProperty for grouping. This datatype property contains all datatype properties for trajectories." ;
  rdfs:domain pi:Trajectory ;
  rdfs:label "Trajectory Property" ;
  rdfs:range xsd:anySimpleType ;
  rdfs:subPropertyOf pi:InfrastructuralFunctionProperty ;
.
pi:Transshipment
  a owl:Class ;
  rdfs:comment "An intermediate destination for transiting cargo to another destination." ;
  rdfs:label "Transshipment" ;
  rdfs:subClassOf pi:LogisticalFunction ;
.
pi:Warehouse
  a owl:Class ;
  rdfs:comment "A place where cargo or its content (products) is stored for a longer period of time" ;
  rdfs:label "Warehouse" ;
  rdfs:subClassOf pi:LogisticalFunction ;
.
pi:BuildingNumber
  a owl:DatatypeProperty ;
  rdfs:comment "this property relates an address to its building number given as string." ;
  rdfs:domain pi:Address ;
  rdfs:label "Building Number" ;
  rdfs:range xsd:string ;
  rdfs:subPropertyOf pi:locationProperties ;
.
pi:cityLoCode
  a owl:DatatypeProperty ;
  rdfs:comment "Code uniquely identifying a City following the LoCode standard." ;
  rdfs:domain pi:City ;
  rdfs:label "City LoCode" ;
  rdfs:range xsd:string ;
  rdfs:subPropertyOf pi:locationProperties ;
.
pi:cityName
  a owl:DatatypeProperty ;
  rdfs:label "City Name" ;
  rdfs:domain pi:City ;
  rdfs:range xsd:string ;
  rdfs:subPropertyOf pi:locationProperties ;
.
pi:containsLogisticalInterface
  a owl:ObjectProperty ;
  rdfs:comment "Each object with a logistical function contains some interfaces where the logistic modality may change." ;
  rdfs:domain pi:LogisticalFunction ;
  rdfs:label "contains logistical interface" ;
  rdfs:range pi:LogisticalInterface ;
.
pi:countryISOCode
  a owl:DatatypeProperty ;
  rdfs:comment "This property identifies a country following the ISO2 codelist standard." ;
  rdfs:domain pi:Country ;
  rdfs:label "Country Code ISO2" ;
  rdfs:range xsd:string ;
  rdfs:subPropertyOf pi:locationProperties ;
.
pi:countryISOCodeAlpha3
  a owl:DatatypeProperty ;
  rdfs:comment "ISO 3166-1 alpha-3 codes are three-letter country codes defined in ISO 3166-1, part of the ISO 3166 standard published by the International Organization for Standardization (ISO), to represent countries, dependent territories, and special areas of geographical interest" ;
  rdfs:domain pi:Country ;
  rdfs:label "country ISOCode Alpha3" ;
  rdfs:range xsd:string ;
  rdfs:subPropertyOf pi:locationProperties ;
.
pi:countryISOCodeNumeric
  a owl:DatatypeProperty ;
  rdfs:comment "Numeric country ISOCode" ;
  rdfs:domain pi:Country ;
  rdfs:label "country ISOCode Numeric" ;
  rdfs:range xsd:string ;
  rdfs:subPropertyOf pi:locationProperties ;
.
pi:countryName
  a owl:DatatypeProperty ;
  rdfs:comment "This property contains the human readable name of the country where the specified location is located in." ;
  rdfs:domain pi:Country ;
  rdfs:label "Country Name" ;
  rdfs:range xsd:string ;
  rdfs:subPropertyOf pi:locationProperties ;
.
pi:geonamesReference
  a owl:ObjectProperty ;
  rdfs:comment "Reference to a geonames feature corresponding to the Location that is the domain of this property." ;
  rdfs:domain pi:Location ;
  rdfs:label "Geonames Reference" ;
  rdfs:range <http://www.geonames.org/ontology#Feature> ;
.
pi:hasCorridorCode
  a owl:ObjectProperty ;
  rdfs:comment "Each corridor has a code, which are collected in the classifications module." ;
  rdfs:domain pi:Corridor ;
  rdfs:label "Has Corridor Code" ;
  rdfs:range classifications:CorridorName ;
.
pi:hasGateNumber
  a owl:DatatypeProperty ;
  rdfs:comment "The number associated with a gate at a logistical function location of type Airport." ;
  rdfs:domain pi:Gate ;
  rdfs:label "Has Gate Number" ;
  rdfs:range xsd:integer ;
  rdfs:subPropertyOf pi:LogisticalInterfaceProperty ;
.
pi:hasLocationRole
  a owl:ObjectProperty ;
  rdfs:comment "This property describes the role a location plays in the context of an event." ;
  rdfs:domain pi:Location ;
  rdfs:label "Has Location Role" ;
  rdfs:range <https://ontology.tno.nl/logistics/federated/LogisticRoles#LocationRoles> ;
.
pi:hasManager
  a owl:ObjectProperty ;
  rdfs:comment "The organisation that manages a specific logistical function" ;
  rdfs:domain pi:LogisticalFunction ;
  rdfs:label "Has Manager" ;
  rdfs:range BusinessService:LegalPerson ;
.
pi:hasOperator
  a owl:DatatypeProperty ;
  rdfs:label "Has Operator" ;
.
pi:hasPlatformNumber
  a owl:DatatypeProperty ;
  rdfs:comment "The number associated with a platform at a logistical function location of type RailwayStation." ;
  rdfs:label "Has Platform Number" ;
  rdfs:subPropertyOf pi:LogisticalInterfaceProperty ;
.
pi:hasQuayNumber
  a owl:DatatypeProperty ;
  rdfs:comment "The number associated with a quay at a logistical function location of type Port." ;
  rdfs:domain pi:Quay ;
  rdfs:label "Has Quay Number" ;
  rdfs:range xsd:integer ;
  rdfs:subPropertyOf pi:LogisticalInterfaceProperty ;
.
pi:locatedAt
  a owl:ObjectProperty ;
  rdfs:comment "This property specifies the geographical location that a Logistical Function has." ;
  rdfs:domain pi:LogisticalFunction ;
  rdfs:label "Located At" ;
  rdfs:range <http://www.w3.org/2003/01/geo/wgs84_pos#SpatialThing> ;
.
pi:locationProperties
  a owl:DatatypeProperty ;
  rdfs:comment "Do not Instantiate. Only for the purpose of grouping. Each subproperty specifies a property of a location." ;
  rdfs:domain pi:Location ;
  rdfs:label "Location Properties" ;
.
pi:logisticalFunctionProperties
  a owl:DatatypeProperty ;
  rdfs:comment "This abstract property contains all properties intended for logistical functions." ;
  rdfs:domain pi:LogisticalFunction ;
  rdfs:label "Logistical Function Properties" ;
  rdfs:range xsd:anySimpleType ;
.
pi:portNumber
  a owl:DatatypeProperty ;
  rdfs:comment "The identification number associated with a specific port." ;
  rdfs:domain pi:Port ;
  rdfs:label "Port Number" ;
  rdfs:range xsd:integer ;
  rdfs:subPropertyOf pi:logisticalFunctionProperties ;
.
pi:portSecurityLevel
  a owl:DatatypeProperty ;
  rdfs:comment "This property specifies the port security level of this specific port." ;
  rdfs:domain pi:Port ;
  rdfs:label "Port Security Level" ;
  rdfs:range xsd:string ;
  rdfs:subPropertyOf pi:logisticalFunctionProperties ;
.
pi:postalCode
  a owl:DatatypeProperty ;
  rdfs:comment "This property specific the postal code or ZIP code of the location involved." ;
  rdfs:domain pi:City ;
  rdfs:label "Postal Code" ;
  rdfs:range xsd:string ;
  rdfs:subPropertyOf pi:locationProperties ;
.
pi:roadName
  a owl:DatatypeProperty ;
  rdfs:comment "This property specifies the name of a road." ;
  rdfs:domain pi:Road ;
  rdfs:label "Road Name" ;
  rdfs:range xsd:string ;
  rdfs:subPropertyOf pi:TrajectoryProperty ;
.
pi:securityMeasure
  a owl:DatatypeProperty ;
  rdfs:comment "This property specifies the security measures of a specific infrastuctural function." ;
  rdfs:domain pi:InfrastructuralFunction ;
  rdfs:label "Security Measure" ;
  rdfs:range xsd:string ;
  rdfs:subPropertyOf pi:InfrastructuralFunctionProperty ;
.
pi:StreetName
  a owl:DatatypeProperty ;
  rdfs:comment "The property that relates an address to its street name given as string." ;
  rdfs:domain pi:Address ;
  rdfs:label "street name" ;
  rdfs:range xsd:string ;
  rdfs:subPropertyOf pi:locationProperties ;
.
pi:terminalDescription
  a owl:DatatypeProperty ;
  rdfs:domain pi:Terminal ;
  rdfs:label "terminal Description" ;
  rdfs:range xsd:string ;
  rdfs:subPropertyOf pi:terminalProperties ;
.
pi:terminalName
  a owl:DatatypeProperty ;
  rdfs:domain pi:Terminal ;
  rdfs:label "terminal Name" ;
  rdfs:range xsd:string ;
  rdfs:subPropertyOf pi:terminalProperties ;
.
pi:terminalProperties
  a owl:DatatypeProperty ;
  rdfs:comment "[for grouping not instantiation] abstract property defined as superProeprty to group terminal data properties." ;
  rdfs:domain pi:Terminal ;
  rdfs:label "terminal Properties" ;
.
