<<<<<<< HEAD
# baseURI: https://ontology.tno.nl/logistics/federated/PhysicalInfrastructure
# imports: http://www.geonames.org/ontology
# imports: http://www.w3.org/2004/02/skos/core
# imports: https://ontology.tno.nl/logistics/federated/BusinessService
# imports: https://ontology.tno.nl/logistics/federated/Classifications
# imports: https://ontology.tno.nl/logistics/federated/DigitalTwin
# imports: https://ontology.tno.nl/logistics/federated/EraAlignment
# imports: https://ontology.tno.nl/logistics/federated/Event
# imports: https://ontology.tno.nl/logistics/federated/LogisticsRoles
# imports: https://ontology.tno.nl/logistics/federated/ReusableTags
# prefix: pi

@prefix : <https://ontology.tno.nl/logistics/federated/PhysicalInfrastructure#> .
@prefix BusinessService: <https://ontology.tno.nl/logistics/federated/BusinessService#> .
@prefix DigitalTwin: <https://ontology.tno.nl/logistics/federated/DigitalTwin#> .
@prefix EraAlignment: <https://ontology.tno.nl/logistics/federated/EraAlignment#> .
@prefix Event: <https://ontology.tno.nl/logistics/federated/Event#> .
@prefix ReusableTags: <https://ontology.tno.nl/logistics/federated/ReusableTags#> .
@prefix classifications: <https://ontology.tno.nl/logistics/federated/Classifications#> .
@prefix owl: <http://www.w3.org/2002/07/owl#> .
@prefix pi: <https://ontology.tno.nl/logistics/federated/PhysicalInfrastructure#> .
@prefix rdf: <http://www.w3.org/1999/02/22-rdf-syntax-ns#> .
@prefix rdfs: <http://www.w3.org/2000/01/rdf-schema#> .
@prefix sh: <http://www.w3.org/ns/shacl#> .
@prefix skos: <http://www.w3.org/2004/02/skos/core#> .
@prefix xsd: <http://www.w3.org/2001/XMLSchema#> .
@prefix dc: <http://purl.org/dc/elements/1.1/> .
@prefix dcterms: <http://purl.org/dc/terms/> .

<https://ontology.tno.nl/logistics/federated/PhysicalInfrastructure>
  rdf:type owl:Ontology ;
  owl:imports <http://www.geonames.org/ontology> ;
  owl:imports <http://www.w3.org/2004/02/skos/core> ;
  owl:imports <https://ontology.tno.nl/logistics/federated/BusinessService> ;
  owl:imports <https://ontology.tno.nl/logistics/federated/Classifications> ;
  owl:imports <https://ontology.tno.nl/logistics/federated/DigitalTwin> ;
  owl:imports <https://ontology.tno.nl/logistics/federated/EraAlignment> ;
  owl:imports <https://ontology.tno.nl/logistics/federated/Event> ;
  owl:imports <https://ontology.tno.nl/logistics/federated/LogisticsRoles> ;
  owl:imports <https://ontology.tno.nl/logistics/federated/ReusableTags> ;
  dc:creator "Dena Tahvildari, Maaike Burghoorn, Cornelis Bouter" ;
  dcterms:description "This ontology contains classes, attributes, relation about physical infrastructure objects that are used in Logistics Events. ;
  dcterms:isRequiredBy <https://ontology.tno.nl/logistics/federated/Event> ;
  dcterms:requires <https://ontology.tno.nl/logistics/federated/Classifications> ;
  dcterms:language "en";
  owl:versionIRI <https://ontology.tno.nl/logistics/federated/PhysicalInfrastructurev-0.1> ;
  dcterms:issued "2021-03-15" ;
  dcterms:created "2020-07-17";
.
pi:Airport
  rdf:type owl:Class ;
  rdfs:comment "Location where airplanes pick or drop off freight." ;
  rdfs:label "Airport" ;
  rdfs:subClassOf pi:LogisticalFunction ;
.
pi:Anchorage
  rdf:type owl:Class ;
  rdfs:comment "A location where a ship can 'park'." ;
  rdfs:label "Anchorage" ;
  rdfs:subClassOf pi:LogisticalFunction ;
.
pi:BargeTerminal
  rdf:type owl:Class ;
  rdfs:comment "A terminal with main modality waterways where cargo of barges can be loaded/discharged." ;
  rdfs:label "Barge Terminal" ;
  rdfs:subClassOf pi:LogisticalFunction ;
.
pi:Bridge
  rdf:type owl:Class ;
  rdfs:comment "A road crossing water." ;
  rdfs:label "Bridge" ;
  rdfs:subClassOf pi:InfrastructuralObject ;
.
pi:City
  rdf:type owl:Class ;
  rdfs:comment "A city is one of the various subtypes of Location." ;
  rdfs:label "City" ;
  rdfs:subClassOf pi:Location ;
.
pi:Corridor
  rdf:type owl:Class ;
  rdf:type sh:NodeShape ;
  rdfs:comment "A logistic corridor is a generalised route. It may consist of several modalities. For example, the route between Europoort and Northern Italy is a corridor, since it's a comman and important route." ;
  rdfs:label "Corridor" ;
  rdfs:subClassOf pi:Trajectory ;
.
pi:Country
  rdf:type owl:Class ;
  rdfs:comment "A Country is a geographic division with national borders." ;
  rdfs:label "Country" ;
  rdfs:subClassOf pi:Location ;
.
pi:DropOffLocation
  rdfs:label "Drop Off Location" ;
.
pi:Gate
  rdf:type owl:Class ;
  rdfs:comment "An interface between road and air." ;
  rdfs:label "Gate" ;
  rdfs:subClassOf pi:LogisticalInterface ;
.
pi:Hub
  rdf:type owl:Class ;
  rdfs:comment "A place where cargo is exchanged between vehicles or/and between transport modes." ;
  rdfs:label "Hub" ;
  rdfs:subClassOf pi:LogisticalFunction ;
.
pi:InfrastructuralFunction
  rdf:type owl:Class ;
  rdfs:comment "Any part of an infrastructure used for performing logistical activities." ;
  rdfs:label "Infrastructural Function" ;
  owl:disjointWith pi:LogisticalFunction ;
.
pi:InfrastructuralObject
  rdf:type owl:Class ;
  rdfs:comment "Any element in an infrastructure that might cause for a delay (e.g. bridge, lock)." ;
  rdfs:label "Infrastructural Object" ;
  rdfs:subClassOf pi:InfrastructuralFunction ;
.
pi:InfrastructurelFunctionProperty
  rdf:type owl:DatatypeProperty ;
  rdfs:comment "A super property for all properties related to infrastructural functions. -- Abstract property, do not instantiate." ;
  rdfs:label "Infrastructural Function Property" ;
.
pi:InlandTerminal
  rdf:type owl:Class ;
  rdfs:comment "An Inland Terminal can have an interface with more than one modality like inland waterways, rail and/or road (note: there are also inland terminals that have only road as modality (e.g. Interporto Bologna) or road and rail (e.g. Zaragoza Logistics Center)." ;
  rdfs:label "Inland Terminal" ;
  rdfs:subClassOf pi:LogisticalFunction ;
.
pi:Landmark
  rdf:type owl:Class ;
  rdfs:comment "A Land Mark is a an object or feature of a landscape or town that is easily recognised from a distance." ;
  rdfs:label "Land Mark" ;
  rdfs:subClassOf pi:Location ;
.
pi:Lat
  rdf:type owl:DatatypeProperty ;
  rdfs:comment "This property specifies the latitude of a specific location." ;
  rdfs:domain pi:Location ;
  rdfs:label "Latitude" ;
  rdfs:range xsd:decimal ;
  rdfs:subPropertyOf pi:LocationCoordinate ;
.
pi:Location
  rdf:type owl:Class ;
  rdfs:comment "A geographical location where several objects with various logistical functions may be." ;
  rdfs:label "Location" ;
  rdfs:subClassOf [
      rdf:type owl:Restriction ;
      owl:minQualifiedCardinality "1"^^xsd:nonNegativeInteger ;
      owl:onDataRange xsd:string ;
      owl:onProperty pi:Lat ;
    ] ;
  rdfs:subClassOf [
      rdf:type owl:Restriction ;
      owl:minQualifiedCardinality "1"^^xsd:nonNegativeInteger ;
      owl:onDataRange xsd:string ;
      owl:onProperty pi:Long ;
    ] ;
  rdfs:subClassOf [
      rdf:type owl:Restriction ;
      owl:minQualifiedCardinality "1"^^xsd:nonNegativeInteger ;
      owl:onDataRange xsd:string ;
      owl:onProperty pi:cityLoCode ;
    ] ;
  rdfs:subClassOf [
      rdf:type owl:Restriction ;
      owl:minQualifiedCardinality "1"^^xsd:nonNegativeInteger ;
      owl:onDataRange xsd:string ;
      owl:onProperty pi:countryISOCode ;
    ] ;
  rdfs:subClassOf [
      rdf:type owl:Restriction ;
      owl:minQualifiedCardinality "1"^^xsd:nonNegativeInteger ;
      owl:onDataRange xsd:string ;
      owl:onProperty pi:countryName ;
    ] ;
  rdfs:subClassOf [
      rdf:type owl:Restriction ;
      owl:minQualifiedCardinality "1"^^xsd:nonNegativeInteger ;
      owl:onDataRange xsd:string ;
      owl:onProperty pi:postalCode ;
    ] ;
.
pi:LocationCoordinate
  rdf:type owl:DatatypeProperty ;
  rdfs:comment "The subproperties of this property specify the location coordinates of a specific location." ;
  rdfs:domain pi:Location ;
  rdfs:label "Location Coordinate" ;
  rdfs:range xsd:decimal ;
.
pi:LogisticalFunction
  rdf:type owl:Class ;
  rdfs:comment "Any location where a logistical activity is performed. A single location may have several logistical functions." ;
  rdfs:label "Logistical Function" ;
.
pi:LogisticalInterface
  rdf:type owl:Class ;
  rdfs:comment "An interface where the modality of a transport may change." ;
  rdfs:label "Logistical Interface" ;
.
pi:LogisticalInterfaceProperty
  rdf:type owl:DatatypeProperty ;
  rdfs:comment "A datatype property for a logistical interface. -- Abstract property, do not instantiate." ;
  rdfs:label "Logistical Interface Property" ;
.
pi:Long
  rdf:type owl:DatatypeProperty ;
  rdfs:comment "This property specifies the longitude of a specific location." ;
  rdfs:domain pi:Location ;
  rdfs:label "Longitude" ;
  rdfs:range xsd:decimal ;
  rdfs:subPropertyOf pi:LocationCoordinate ;
.
pi:PickUpLocation
  rdfs:label "Pickup Location" ;
.
pi:PlaceOfArrival
  rdfs:comment "A place of a call of a transport means following (in time) the last place of departure (milestone value is departure)" ;
  rdfs:label "Place of Departure" ;
.
pi:PlaceOfCall
  rdfs:label "Place of Call" ;
.
pi:Platform
  rdf:type owl:Class ;
  rdfs:comment "An interface to or from the Railway modality." ;
  rdfs:label "Platform" ;
  rdfs:subClassOf pi:LogisticalInterface ;
.
pi:Port
  rdf:type owl:Class ;
  rdfs:comment "Location where vessels pick or drop off freight." ;
  rdfs:label "Port" ;
  rdfs:subClassOf pi:LogisticalFunction ;
.
pi:Quay
  rdf:type owl:Class ;
  rdfs:comment "An interface to or from sea and inland waterways." ;
  rdfs:label "Quay" ;
  rdfs:subClassOf pi:LogisticalInterface ;
.
pi:RailwayLine
  rdf:type owl:Class ;
  rdfs:comment "A trajectory with modality 'rail'." ;
  rdfs:label "Railway Line" ;
  rdfs:subClassOf pi:Trajectory ;
.
pi:RailwayStation
  rdf:type owl:Class ;
  rdfs:comment "A location where railway wagons and locomotives drop off or pick up freight." ;
  rdfs:label "Railway Station" ;
  rdfs:subClassOf pi:InlandTerminal ;
.
pi:RailwayTerminal
  rdf:type owl:Class ;
  rdfs:comment "An inland terminal managed by a railway infrastructure manager with main modality rail." ;
  rdfs:label "Railway Terminal" ;
  rdfs:subClassOf pi:InlandTerminal ;
.
pi:Road
  rdf:type owl:Class ;
  rdfs:comment "A trajectory with modality 'road'." ;
  rdfs:label "Road" ;
  rdfs:subClassOf pi:Trajectory ;
.
pi:Terminal
  rdf:type owl:Class ;
  rdfs:comment "A location interfacing with main modality sea." ;
  rdfs:label "Terminal" ;
  rdfs:subClassOf pi:Hub ;
.
pi:Trajectory
  rdf:type owl:Class ;
  rdfs:comment "Any part of an infrastructure identified by its infrastructure manager." ;
  rdfs:label "Trajectory" ;
.
pi:TrajectoryProperty
  rdf:type owl:DatatypeProperty ;
  rdfs:comment "DO NOT Instantiate -- superProperty for grouping. This datatype property contains all datatype properties for trajectories." ;
  rdfs:domain pi:Trajectory ;
  rdfs:label "Trajectory Property" ;
  rdfs:range xsd:anySimpleType ;
  rdfs:subPropertyOf pi:InfrastructurelFunctionProperty ;
.
pi:Transshipment
  rdf:type owl:Class ;
  rdfs:comment "An intermediate destination for transiting cargo to another destination." ;
  rdfs:label "Transshipment" ;
  rdfs:subClassOf pi:LogisticalFunction ;
.
pi:Warehouse
  rdf:type owl:Class ;
  rdfs:comment "A place where cargo or its content (products) is stored for a longer period of time" ;
  rdfs:label "Warehouse" ;
  rdfs:subClassOf pi:LogisticalFunction ;
.
pi:cityLoCode
  rdf:type owl:DatatypeProperty ;
  rdfs:comment "Code uniquely identifying a City following the LoCode standard." ;
  rdfs:domain pi:City ;
  rdfs:label "City LoCode" ;
  rdfs:range xsd:string ;
  rdfs:subPropertyOf pi:locationProperties ;
.
pi:cityName
  rdf:type owl:DatatypeProperty ;
  rdfs:label "Has Manager" ;
  rdfs:subPropertyOf pi:locationProperties ;
.
pi:countryISOCode
  rdf:type owl:DatatypeProperty ;
  rdfs:comment "This property identifies a country following the ISO2 codelist standard." ;
  rdfs:domain pi:Location ;
  rdfs:label "Country Code iso2" ;
  rdfs:range xsd:string ;
  rdfs:subPropertyOf pi:locationProperties ;
.
pi:countryName
  rdf:type owl:DatatypeProperty ;
  rdfs:comment "This property contains the human readable name of the country where the specified location is located in." ;
  rdfs:domain pi:Location ;
  rdfs:label "Country Name" ;
  rdfs:range xsd:string ;
  rdfs:subPropertyOf pi:locationProperties ;
.
pi:geonamesReference
  rdf:type owl:ObjectProperty ;
  rdfs:comment "Reference to a geonames feature corresponding to the Location that is the domain of this property." ;
  rdfs:domain pi:Location ;
  rdfs:label "Geonames Feature" ;
  rdfs:range <http://www.geonames.org/ontology#Feature> ;
.
pi:hasCorridorCode
  rdf:type owl:ObjectProperty ;
  rdfs:comment "Each corridor has a code, which are collected in the classifications module." ;
  rdfs:domain pi:Corridor ;
  rdfs:label "Has Corridor Code" ;
  rdfs:range classifications:CorridorName ;
.
pi:hasGateNumber
  rdf:type owl:DatatypeProperty ;
  rdfs:comment "The number associated with a gate at a logistical function location of type Airport." ;
  rdfs:domain pi:Gate ;
  rdfs:label "Has Gate Number" ;
  rdfs:range xsd:integer ;
  rdfs:subPropertyOf pi:LogisticalInterfaceProperty ;
.
pi:hasLocationRole
  rdf:type owl:ObjectProperty ;
  rdfs:comment "This property describes the role a location plays in the context of an event." ;
  rdfs:domain pi:Location ;
  rdfs:label "Has Location Role" ;
  rdfs:range <https://ontology.tno.nl/logistics/federated/LogisticsRoles#LocationRoles> ;
.
pi:hasManager
  rdf:type owl:ObjectProperty ;
  rdfs:comment "The organisation that manages a specific logistical function" ;
  rdfs:domain pi:LogisticalFunction ;
  rdfs:label "Has Manager" ;
  rdfs:range BusinessService:LogisticsActor ;
.
pi:hasOperator
  rdf:type owl:DatatypeProperty ;
  rdfs:label "Has Operator" ;
.
pi:hasPlatformNumber
  rdf:type owl:DatatypeProperty ;
  rdfs:comment "The number associated with a platform at a logistical function location of type RailwayStation." ;
  rdfs:label "Has Platform Number" ;
  rdfs:subPropertyOf pi:LogisticalInterfaceProperty ;
.
pi:hasQuayNumber
  rdf:type owl:DatatypeProperty ;
  rdfs:comment "The number associated with a quay at a logistical function location of type Port." ;
  rdfs:domain pi:Quay ;
  rdfs:label "Has Quay Number" ;
  rdfs:range xsd:integer ;
  rdfs:subPropertyOf pi:LogisticalInterfaceProperty ;
.
pi:locatedAt
  rdf:type owl:ObjectProperty ;
  rdfs:comment "This property specifies the geographical location that a Logistical Function has." ;
  rdfs:domain pi:LogisticalFunction ;
  rdfs:label "Located At" ;
  rdfs:range pi:Location ;
.
pi:locationProperties
  rdf:type owl:DatatypeProperty ;
  rdfs:comment "Do not Instantiate. Only for the purpose of grouping. Each subproperty specifies a property of a location." ;
  rdfs:domain pi:Location ;
  rdfs:label "Location Properties" ;
  rdfs:range xsd:anySimpleType ;
.
pi:logisticalFunctionProperties
  rdf:type owl:DatatypeProperty ;
  rdfs:comment "This abstract property contains all properties intended for logistical functions." ;
  rdfs:domain pi:LogisticalFunction ;
  rdfs:label "Logistical Function Properties" ;
  rdfs:range xsd:anySimpleType ;
.
pi:placeOfAcceptance
  rdfs:comment "Place at which the goods are taken over by the carrier." ;
  rdfs:label "Place of Acceptance" ;
.
pi:placeOfBorderCrossing
  rdfs:comment "A place where a new customs domain is entered by a transport means during its itinerary " ;
  rdfs:label "Place of Departure" ;
.
pi:placeOfDelivery
  rdfs:comment "Place to which the goods are to be finally delivered under transport contract terms (operational term)." ;
  rdfs:label "City" ;
.
pi:placeOfDeparture
  rdfs:comment "A place where a transport means arrived (milestone value: arrival) and is able to depart." ;
  rdfs:label "Place of Departure" ;
.
pi:placeOfLoading
  rdfs:comment "Seaport, airport, freight terminal, rail station or other place at which the goods (cargo) are loaded on to the means of transport being used for their carriage." ;
  rdfs:label "Place of Departure" ;
.
pi:placeOfReceipt
  rdfs:comment "A place of receipt is the place where the cargo is offered for transport by a business transaction to the service provider that is the carrier and has to be transported by that carrier to the place of loading of the main transport. The cargo has to be at that location." ;
  rdfs:label "Place of Receipt" ;
.
pi:placeOfUnloading
  rdfs:comment "A place of unloading is the place to where the cargo has to be transported by a business transaction to the service provider that is the carrier and will be discharged/unloaded from that transport means. The cargo and the transport means have to be at that location." ;
  rdfs:label "Place of Departure" ;
.
pi:portNumber
  rdf:type owl:DatatypeProperty ;
  rdfs:comment "The identification number associated with a specific port." ;
  rdfs:domain pi:Port ;
  rdfs:label "Port Number" ;
  rdfs:range xsd:integer ;
  rdfs:subPropertyOf pi:logisticalFunctionProperties ;
.
pi:portSecurityLevel
  rdf:type owl:DatatypeProperty ;
  rdfs:comment "This property specifies the port security level of this specific port." ;
  rdfs:domain pi:Port ;
  rdfs:label "Port Security Level" ;
  rdfs:lable "Port Security Level" ;
  rdfs:range xsd:string ;
  rdfs:subPropertyOf pi:logisticalFunctionProperties ;
.
pi:postalCode
  rdf:type owl:DatatypeProperty ;
  rdfs:comment "This property specific the postal code or ZIP code of the location involved." ;
  rdfs:domain pi:Location ;
  rdfs:label "Postal Code" ;
  rdfs:range xsd:string ;
  rdfs:subPropertyOf pi:locationProperties ;
.
pi:roadName
  rdf:type owl:DatatypeProperty ;
  rdfs:comment "This property specifies the name of a road." ;
  rdfs:domain pi:Road ;
  rdfs:label "Road Name" ;
  rdfs:range xsd:string ;
  rdfs:subPropertyOf pi:TrajectoryProperty ;
.
pi:securityMeasure
  rdf:type owl:DatatypeProperty ;
  rdfs:comment "This property specifies the security measures of a specific infrastuctural function." ;
  rdfs:domain pi:InfrastructuralFunction ;
  rdfs:label "Security Measure" ;
  rdfs:range xsd:string ;
  rdfs:subPropertyOf pi:logisticalFunctionProperties ;
.